execution_invariants_s.thy
@@ -115,8 +115,8 @@ next
   from \<open>S ~~ (i, a) \<leadsto>\<^sub>S S'\<close>
   show ?case 
   proof (induct rule: step_s.cases)
-    case (local C s ls f ls')
-    then have "S ~~ (i, ALocal) \<leadsto> S'"
+    case (local C s ls f ok ls')
+    then have "S ~~ (i, ALocal ok) \<leadsto> S'"
       by (auto simp add: step_simps)
     then show ?case
       using state_wellFormed_combine_step step.IH by fastforce 
