packed_nofails_noinvchecks.thy
@@ -1,6 +1,8 @@
 section "Packed Traces without Failures and Invariant Checks"
 theory packed_nofails_noinvchecks
-imports no_failing_invchecks packed_no_fails consistency
+  imports no_failing_invchecks packed_no_fails consistency single_invocation_reduction_helper
+"fuzzyrule.fuzzyrule"
+state_monotonicGrowth_invariants
 begin
 
 
@@ -165,7 +167,7 @@ proof (rule show_programCorrect_noTransactionInterleaving)
         by  (auto simp add: trace'_def isNotTrueInvcheck_def)
     qed
     then have "traceCorrect trace"
-      by (auto simp add: trace'_def traceCorrect_def isNotTrueInvcheck_def)
+      by  (auto simp add: trace'_def traceCorrect_def isNotTrueInvcheck_def actionCorrect_def, force+)
 
     then show "False"
       using a by blast
@@ -499,7 +501,7 @@ text \<open>
 \<close>
 theorem show_programCorrect_noTransactionInterleaving':
   assumes packedTracesCorrect: 
-    "\<And>trace s. \<lbrakk>initialState program ~~ trace \<leadsto>* s; packed_trace trace; \<And>s. (s, ACrash) \<notin> set trace; no_invariant_checks_in_transaction trace\<rbrakk> \<Longrightarrow> traceCorrect trace"
+    "\<And>trace s. \<lbrakk>initialState program ~~ trace \<leadsto>* s; packed_trace trace; \<And>s. (s, ACrash) \<notin> set trace; \<And>s. (s, AInvcheck True) \<notin> set trace; no_invariant_checks_in_transaction trace\<rbrakk> \<Longrightarrow> traceCorrect trace"
   shows "programCorrect program"
 proof (rule show_programCorrect_noTransactionInterleaving_no_passing_invchecks)
   fix trace
@@ -512,498 +514,1520 @@ proof (rule show_programCorrect_noTransactionInterleaving_no_passing_invchecks)
 
 
   show "traceCorrect trace"
-  proof (rule ccontr)
-    assume a: "\<not> traceCorrect trace"
-
-    \<comment> \<open>get the first failing invariant check\<close>
-    obtain i 
-      where i1: "\<exists>s. trace ! i = (s, AInvcheck False)"
-        and i2: "i < length trace"
-        and i_min: "\<forall>i'. (\<exists> s'. trace ! i' = (s', AInvcheck False)) \<and> i' < length trace \<longrightarrow> i\<le>i'"
-      by (atomize_elim,
-       rule exI[where x="LEAST i'. (\<exists>s'. trace ! i' = (s', AInvcheck False)) \<and> i' < length trace"],
-       rule LeastI2_wellorder_ex,
-       insert a,
-       auto simp add: traceCorrect_def in_set_conv_nth)
-
-    from i1
-    obtain s where i1': "trace ! i = (s, AInvcheck False)"
-      by blast
-
-    have trace_split3: "trace = take (Suc i) trace  @ drop (Suc i) trace"
-      by auto
-
-    with steps
-    have "initialState program ~~ take (Suc i) trace  @ drop (Suc i) trace \<leadsto>* S" 
-      by simp
+  proof (cases "\<exists>a\<in>set trace. get_action a = AInvcheck False")
+    case True
     from this
-    obtain Si 
-      where steps_Si: "initialState program ~~ take (Suc i) trace \<leadsto>* Si"
+    obtain i1 where exists_inv_fail: "(\<exists>s. trace!i1 = (s, AInvcheck False)) \<and> i1 < length trace" 
+      by (metis eq_snd_iff in_set_conv_nth)
+
+
+    show "traceCorrect trace"
+    proof (rule ccontr)
+      assume a: "\<not> traceCorrect trace"
+
+\<comment> \<open>get the first failing invariant check\<close>
+      obtain i 
+        where i1: "\<exists>s. trace ! i = (s, AInvcheck False)"
+          and i2: "i < length trace"
+          and i_min: "\<forall>i'. (\<exists> s'. trace ! i' = (s', AInvcheck False)) \<and> i' < length trace \<longrightarrow> i\<le>i'"
+        by (atomize_elim,
+            rule exI[where x="LEAST i'. (\<exists>s'. trace ! i' = (s', AInvcheck False)) \<and> i' < length trace"],
+            rule LeastI2_wellorder_ex,
+            insert exists_inv_fail, auto)
+
+
+
+
+      from i1
+      obtain s where i1': "trace ! i = (s, AInvcheck False)"
+        by blast
+
+      have trace_split3: "trace = take (Suc i) trace  @ drop (Suc i) trace"
+        by auto
+
+      with steps
+      have "initialState program ~~ take (Suc i) trace  @ drop (Suc i) trace \<leadsto>* S" 
+        by simp
+      from this
+      obtain Si 
+        where steps_Si: "initialState program ~~ take (Suc i) trace \<leadsto>* Si"
         using steps_append by blast
 
-    have "\<exists>trace' s'. (\<exists>S'. initialState program ~~ trace' \<leadsto>* S') \<and>
+      have "\<exists>trace' s'. (\<exists>S'. initialState program ~~ trace' \<leadsto>* S') \<and>
                   packed_trace trace' \<and>
                   (\<forall>s. (s, ACrash) \<notin> set trace') \<and>
                   (\<forall>s. (s, AInvcheck True) \<notin> set trace') \<and> last trace' = (s', AInvcheck False) \<and> 0 < length trace' \<and> no_invariant_checks_in_transaction trace'"
-    proof (rule  move_invariant_checks_out_of_transactions[OF steps_Si])
-      show "packed_trace (take (Suc i) trace)"
-        by (metis isPrefix_appendI packed prefixes_are_packed trace_split3)
-      show "\<And>s. (s, ACrash) \<notin> set (take (Suc i) trace)"
-        by (meson in_set_takeD nofail)
-      show "\<And>s. (s, AInvcheck True) \<notin> set (take (Suc i) trace)"
-        by (meson in_set_takeD noTrueInvs)
-      show "last (take (Suc i) trace) = (s, AInvcheck False)"
-        by (simp add: i1' i2 take_Suc_conv_app_nth)
-      show "0 < length (take (Suc i) trace)"
-        using gr_implies_not_zero i2 by auto
-      show "\<And>ia s' . ia < length (take (Suc i) trace) - 1 \<Longrightarrow> take (Suc i) trace ! ia \<noteq> (s', AInvcheck False)"
-        using i_min by fastforce
-    qed
+      proof (rule  move_invariant_checks_out_of_transactions[OF steps_Si])
+        show "packed_trace (take (Suc i) trace)"
+          by (metis isPrefix_appendI packed prefixes_are_packed trace_split3)
+        show "\<And>s. (s, ACrash) \<notin> set (take (Suc i) trace)"
+          by (meson in_set_takeD nofail)
+        show "\<And>s. (s, AInvcheck True) \<notin> set (take (Suc i) trace)"
+          by (meson in_set_takeD noTrueInvs)
+        show "last (take (Suc i) trace) = (s, AInvcheck False)"
+          by (simp add: i1' i2 take_Suc_conv_app_nth)
+        show "0 < length (take (Suc i) trace)"
+          using gr_implies_not_zero i2 by auto
+        show "\<And>ia s' . ia < length (take (Suc i) trace) - 1 \<Longrightarrow> take (Suc i) trace ! ia \<noteq> (s', AInvcheck False)"
+          using i_min by fastforce
+      qed
 
-    then show False
-      by (auto,
-          metis last_in_set packedTracesCorrect traceCorrect_def)
+      then show False
+        using actionCorrect_def last_in_set packedTracesCorrect traceCorrect_def by fastforce
+    qed
+  next 
+    case False
+    show ?thesis
+      using steps
+    proof (rule packedTracesCorrect)
+      show "packed_trace trace"
+        by (simp add: packed)
+
+      show "\<And>s. (s, ACrash) \<notin> set trace"
+        by (simp add: nofail)
+
+      show "\<And>s. (s, AInvcheck True) \<notin> set trace"
+        by (simp add: noTrueInvs)
+
+
+      show "no_invariant_checks_in_transaction trace"
+        using False noTrueInvs 
+        by (auto simp add: no_invariant_checks_in_transaction_def all_set_conv_all_nth in_set_conv_nth)
+    qed
   qed
 qed
+
+(* TODO utils *)
+lemma show_list_split:
+  assumes "ys = take (length ys) xs"
+    and "zs = drop (length ys) xs"
+  shows "xs = ys @ zs"
+  by (metis append_take_drop_id assms(1) assms(2))
+
+lemma append_eq_conv_conj':
+  shows "(xs = ys @ zs) \<longleftrightarrow> (ys = take (length ys) xs \<and> zs = drop (length ys) xs)"
+  by (metis append_eq_conv_conj)
+
+lemma cons_eq_conv_conj': 
+  "(y # ys = xs) \<longleftrightarrow> (xs \<noteq> [] \<and> y = hd xs \<and> ys = tl xs)"  for xs ys zs
+  by force
+
+lemmas list_split_utils = 
+  append_eq_conv_conj 
+  append_eq_conv_conj'
+  cons_eq_conv_conj 
+  cons_eq_conv_conj'
+
+lemma min_simps:
+  fixes x :: nat
+  shows
+ "x < y \<Longrightarrow> min x y = x"
+"x < y \<Longrightarrow> min y x = x"
+ "x \<le> y \<Longrightarrow> min x y = x"
+"x \<le> y \<Longrightarrow> min y x = x"
+  by auto
+
+
+lemma no_more_actions_on_packed_trace_if_context_switch_in_transaction:
+  assumes "S ~~ tr \<leadsto>* S'"
+    and "packed_trace tr"
+    and "currentTransaction S i \<triangleq> tx"
+    and "get_invoc (hd tr) \<noteq> i"
+    and "tr \<noteq> []"
+    and "state_wellFormed S"
+    and "\<And>i. (i, ACrash) \<notin> set tr"
+  shows "currentTransaction S' i \<triangleq> tx \<and> (\<forall>a\<in>set tr. get_invoc a \<noteq> i)"
+  using assms proof (induct rule: steps_induct)
+  case initial
+  then show ?case
+    by simp
+next
+  case (step S' tr a S'')
+
+  show ?case
+  proof (cases tr)
+    case Nil
+    then show ?thesis
+      using step by (auto simp add: steps_empty,
+          metis prod.collapse unchangedInTransaction(3))
+  next
+    case (Cons x xs)
+
+
+
+
+    have IH: "currentTransaction S' i \<triangleq> tx \<and> (\<forall>a\<in>set tr. get_invoc a \<noteq> i)"
+    proof (rule step.IH)
+      show "packed_trace tr"
+        using packed_trace_prefix step.prems(1) by blast
+      show "currentTransaction S i \<triangleq> tx"
+        by (simp add: step.prems(2))
+      show "tr \<noteq> []"
+        using local.Cons by blast
+      show " get_invoc (hd tr) \<noteq> i"
+        using \<open>tr \<noteq> []\<close> step.prems(3) by auto
+      show "state_wellFormed S"
+        by (simp add: step.prems(5))
+      show "\<And>i. (i, ACrash) \<notin> set tr"
+        using step.prems(6) by auto
+
+    qed
+
+    have "state_wellFormed S'"
+      using state_wellFormed_combine
+        `S ~~ tr \<leadsto>* S'` `state_wellFormed S`
+        step.prems(6) by fastforce 
+
+
+
+    from use_packed_trace[OF `packed_trace (tr @ [a])`, where i="length tr"]
+    have no_context_switch: "allowed_context_switch (get_action a)" if "get_invoc a = i"
+      by (auto, metis IH diff_Suc_less length_greater_0_conv list.distinct(1) local.Cons nth_append nth_mem that)
+
+    find_theorems allowed_context_switch packed_trace
+
+
+    from `S' ~~ a \<leadsto> S''` IH no_context_switch
+    show ?thesis
+      using  state_wellFormed_ls_to_visibleCalls[OF \<open>state_wellFormed S'\<close>]
+      by (auto simp add: step.simps allowed_context_switch_def, blast)
+
+
+
+  qed
+qed
+
+lemma no_invariant_checks_in_transaction_prefix:
+  assumes a: "no_invariant_checks_in_transaction tr"
+and p: "isPrefix tr' tr"
+shows "no_invariant_checks_in_transaction tr'"
+  using a isPrefix_len[OF p] isPrefix_same[OF p] order.strict_trans2
+  by (auto simp add: no_invariant_checks_in_transaction_def, blast)
+
+lemma no_context_switch_transaction:
+  assumes "S ~~ tr \<leadsto>* S'"
+    and "(hd tr) = (invoc, ABeginAtomic tx txns)"
+    and "(invoc, AEndAtomic) \<notin> set tr"
+    and "packed_trace tr"
+    and "\<forall>a\<in>set (tl tr). \<not>allowed_context_switch (get_action a)"
+  shows "\<forall>a\<in>set tr. get_invoc a = invoc"
+  using assms proof (induct rule: steps_induct)
+  case initial
+  then show ?case
+    by simp
+next
+  case (step S' tr a S'')
+
+  show ?case
+  proof (cases "tr=[]")
+    case True
+    then show ?thesis 
+      using step.prems(1) by auto
+  next
+    case False
+
+
+    have "packed_trace tr"
+      using packed_trace_prefix step.prems(3) by blast
+
+    have "hd tr = (invoc, ABeginAtomic tx txns)" 
+      using step.prems(1) `tr \<noteq> []` by auto
+
+
+    have "(invoc, AEndAtomic) \<notin> set tr"
+      using step.prems(2) by auto
+
+    from step.IH
+    have "\<forall>a\<in>set tr. get_invoc a = invoc"
+      using False \<open>(invoc, AEndAtomic) \<notin> set tr\<close> \<open>hd tr = (invoc, ABeginAtomic tx txns)\<close> \<open>packed_trace tr\<close> step.prems(4) by auto
+
+
+    from `\<forall>a\<in>set (tl (tr @ [a])). \<not> allowed_context_switch (get_action a)`
+    have "\<not>allowed_context_switch (get_action a)" if "tr \<noteq> []"
+      using that by auto
+
+
+
+    have "get_invoc a = invoc"
+    proof (rule ccontr)
+      assume "get_invoc a \<noteq> invoc"
+      hence "allowed_context_switch (get_action a)"
+        using use_packed_trace[OF `packed_trace (tr @ [a])`, where i="length tr"]
+        by (simp add: False \<open>\<forall>a\<in>set tr. get_invoc a = invoc\<close> nth_append)
+
+      thus False
+        using False \<open>tr \<noteq> [] \<Longrightarrow> \<not> allowed_context_switch (get_action a)\<close> by blast
+    qed
+
+
+    show ?thesis
+      using \<open>\<forall>a\<in>set tr. get_invoc a = invoc\<close> \<open>get_invoc a = invoc\<close> by auto
+  qed
+qed
+
+lemma no_context_switch_transaction2:
+  assumes "S ~~ tr \<leadsto>* S'"
+    and "tr!i = (invoc, ABeginAtomic tx txns)"
+    and "\<And>j. i < j \<Longrightarrow> j \<le> k \<Longrightarrow> tr ! j \<noteq> (invoc, AEndAtomic)"
+    and "packed_trace tr"
+    and "\<And>j. i < j \<Longrightarrow> j \<le> k \<Longrightarrow> \<not>allowed_context_switch (get_action (tr!j))"
+    and "i \<le> k"
+    and "k < length tr"
+  shows "get_invoc (tr!k) = invoc"
+proof -
+
+  obtain tr1 tr2 tr3 
+    where tr_split: "tr = tr1 @ tr2 @ tr3"
+      and "i = length tr1"
+      and "length tr1 + length tr2 = Suc k"
+    by (metis Suc_leI append.assoc append_take_drop_id assms(6) assms(7) le_imp_less_Suc length_append length_take less_imp_le min.absorb2)
+
+
+  with `S ~~ tr \<leadsto>* S'`
+  obtain Sa Sb 
+    where "S ~~ tr1 \<leadsto>* Sa"
+      and "Sa ~~ tr2 \<leadsto>* Sb"
+    using steps_append by blast
+
+
+  have [simp]: "tr2 \<noteq> []"
+    using \<open>i = length tr1\<close> \<open>length tr1 + length tr2 = Suc k\<close> assms(6) by auto
+
+  have [simp]: "tr2 ! 0 = (invoc, ABeginAtomic tx txns)"
+    by (metis \<open>i = length tr1\<close> \<open>tr2 \<noteq> []\<close> add.right_neutral assms(2) length_greater_0_conv nth_append_first nth_append_length_plus tr_split)
+  hence [simp]: "hd tr2 = (invoc, ABeginAtomic tx txns)"
+    by (simp add: hd_conv_nth)
+    
+
+  have "\<forall>a\<in>set tr2. get_invoc a = invoc"
+    using `Sa ~~ tr2 \<leadsto>* Sb`
+  proof (rule no_context_switch_transaction)
+    show "hd tr2 = (invoc, ABeginAtomic tx txns)"
+      using `tr!i = (invoc, ABeginAtomic tx txns)`
+      by (auto simp add: tr_split nth_append `i = length tr1` split: if_splits)
+    show "(invoc, AEndAtomic) \<notin> set tr2"
+      using `\<And>j. i < j \<Longrightarrow> j \<le> k \<Longrightarrow> tr ! j \<noteq> (invoc, AEndAtomic)`
+      using \<open>i = length tr1\<close> \<open>length tr1 + length tr2 = Suc k\<close> 
+      apply (auto simp add: tr_split nth_append in_set_conv_nth split: if_splits)
+
+      apply (drule_tac x="length tr1 + ia" in meta_spec)
+      apply (auto simp add: tr_split nth_append in_set_conv_nth split: if_splits)
+      apply (case_tac ia)
+       apply auto
+      done
+    show "packed_trace tr2"
+      using assms(4) packed_trace_postfix packed_trace_prefix tr_split by auto 
+    show "\<forall>a\<in>set (tl tr2). \<not> allowed_context_switch (get_action a)"
+      using `\<And>j. i < j \<Longrightarrow> j \<le> k \<Longrightarrow> \<not>allowed_context_switch (get_action (tr!j))`
+      apply (auto simp add: tr_split nth_append in_set_conv_nth split: if_splits)
+      apply (drule_tac x="length tr1 + ia" in meta_spec)
+      apply (auto simp add: tr_split nth_append in_set_conv_nth nth_tl split: if_splits)
+      by (metis One_nat_def Suc_leI \<open>i = length tr1\<close> \<open>length tr1 + length tr2 = Suc k\<close> add.commute add_Suc_right add_diff_cancel_left' assms(5) less_add_Suc1 less_diff_conv nth_append_first nth_append_length_plus plus_1_eq_Suc snd_conv tr_split)
+  qed
+
+  thus "get_invoc (tr ! k) = invoc"
+    by (metis (no_types, lifting) Suc_diff_le \<open>i = length tr1\<close> \<open>length tr1 + length tr2 = Suc k\<close> add_diff_cancel_left' assms(6) in_set_conv_nth leD lessI nth_append tr_split)
+qed
+
+lemma transfer_execution:
+  assumes steps: "S1 ~~ tr \<leadsto>* S2"
+    and p: "P S1 S1'"
+    and wf: "state_wellFormed S1"
+    and no_crash: "\<And>i. (i, ACrash) \<notin> set tr"
+    and induct: "\<And>a tr' Sa Sb Sa' . \<lbrakk>
+      a\<in>set tr; 
+      P Sa Sa'; 
+      Sa ~~ a \<leadsto> Sb; 
+      state_wellFormed Sa;
+      S1 ~~ tr' \<leadsto>* Sa;
+      isPrefix tr' tr
+    \<rbrakk> \<Longrightarrow> \<exists>Sb'. (Sa' ~~ a \<leadsto> Sb') \<and> P Sb Sb'"
+  shows "\<exists>S2'. (S1' ~~ tr \<leadsto>* S2') \<and> P S2 S2'"
+proof -
+
+  define tr_alt where "tr_alt = tr"
+
+  have "isPrefix tr tr_alt"
+    by (simp add: isPrefix_refl tr_alt_def)
+
+  have induct_alt: "\<And>a tr' Sa Sb Sa' . \<lbrakk>
+      a\<in>set tr_alt; 
+      P Sa Sa'; 
+      Sa ~~ a \<leadsto> Sb; 
+      state_wellFormed Sa;
+      S1 ~~ tr' \<leadsto>* Sa;
+      isPrefix tr' tr_alt
+    \<rbrakk> \<Longrightarrow> \<exists>Sb'. (Sa' ~~ a \<leadsto> Sb') \<and> P Sb Sb'"
+    by (simp add: induct tr_alt_def)
+
+
+  have "\<exists>S2'. (S1' ~~ tr \<leadsto>* S2') \<and> P S2 S2' \<and> isPrefix tr tr_alt "
+    using steps induct_alt no_crash `isPrefix tr tr_alt` proof (induct rule: steps_induct)
+    case initial
+    then show ?case
+      using p by (simp add: steps_empty isPrefix_empty_first)
+
+  next
+    case (step S2 tr a S3)
+
+    have "\<exists>S2'. (S1' ~~ tr \<leadsto>* S2') \<and> P S2 S2' \<and> isPrefix tr tr_alt"
+    proof (rule step.IH)
+      from `isPrefix (tr @ [a]) tr_alt`
+      show "isPrefix tr tr_alt"
+        by (metis append_take_drop_id isPrefix_append isPrefix_appendI isPrefix_def )
+
+      show "\<exists>Sb'. (Sa' ~~ a \<leadsto> Sb') \<and> P Sb Sb'"
+        if c0: "a \<in> set tr_alt"
+          and c1: "P Sa Sa'"
+          and c2: "Sa ~~ a \<leadsto> Sb"
+          and c3: "state_wellFormed Sa"
+          and c4: "S1 ~~ tr' \<leadsto>* Sa"
+          and c5: "isPrefix tr' tr_alt"
+        for  a Sa Sa' Sb tr'
+        using c0 c1 c2 c3 c4 c5 induct_alt by blast
+
+
+
+
+      show " \<And>i. (i, ACrash) \<notin> set tr"
+        using step.prems by auto
+    qed
+
+    from this
+    obtain S2' where "(S1' ~~ tr \<leadsto>* S2')" and "P S2 S2'" and "isPrefix tr tr_alt"
+      by blast
+
+    have "\<exists>S3'. (S2' ~~ a \<leadsto> S3') \<and> P S3 S3'"
+    proof (rule step)
+      from `isPrefix (tr @ [a]) tr_alt`
+      show "a \<in> set tr_alt"
+        by (metis in_set_takeD isPrefix_def list.set_intros(1) rotate1.simps(2) set_rotate1 step.prems(3))
+
+      show "P S2 S2'"
+        using `P S2 S2'` .
+      show "S2 ~~ a \<leadsto> S3"
+        using `S2 ~~ a \<leadsto> S3` .
+      show "state_wellFormed S2"
+        using local.wf state_wellFormed_combine step.prems(2) step.steps by fastforce
+      show "S1 ~~ tr \<leadsto>* S2"
+        by (simp add: step.steps)
+      show "isPrefix tr tr_alt"
+        by (simp add: \<open>isPrefix tr tr_alt\<close>)
+
+    qed
+
+
+    then show ?case
+      using \<open>S1' ~~ tr \<leadsto>* S2'\<close> step.prems(3) steps_step by blast
+  qed
+  thus ?thesis
+    by blast
+qed    
+
+lemma show_state_transfer2:
+  assumes steps: "S1 ~~ tr \<leadsto>* S2"
+    and wf: "state_wellFormed S1"
+    and no_crash: "\<And>i. (i, ACrash) \<notin> set tr"
+    and p: "S1' = f S1"
+    and indu: "\<And>i a Sa Sb tr' . \<lbrakk>
+      (i,a)\<in>set tr; 
+      Sa ~~ (i, a) \<leadsto> Sb; 
+      state_wellFormed Sa;
+      isPrefix tr' tr;
+      S1 ~~ tr' \<leadsto>* Sa
+    \<rbrakk> \<Longrightarrow> f Sa ~~ (i, a) \<leadsto> f Sb"
+  shows "S1' ~~ tr \<leadsto>* f S2"
+proof  -
+
+  from steps p wf no_crash
+  have "\<exists>S2'. (S1' ~~ tr \<leadsto>* S2') \<and> S2' = f S2"
+  proof (rule transfer_execution)
+
+    show "\<exists>Sb'. (Sa' ~~ a \<leadsto> Sb') \<and> Sb' = f Sb"
+      if c0: "a \<in> set tr"
+        and c1: "Sa' = f Sa"
+        and c2: "Sa ~~ a \<leadsto> Sb"
+        and c3: "state_wellFormed Sa"
+        and c4: "S1 ~~ tr' \<leadsto>* Sa"
+        and c5: "isPrefix tr' tr"
+      for  a tr' Sa Sb Sa'
+      by (metis c0 c1 c2 c3 c4 c5 indu prod.collapse)
+  qed
+  thus ?thesis
+    by blast
+qed
+
+
+lemma drop_single_action:
+  assumes step1: "S1 ~~ ia \<leadsto> S2" 
+    and steps: "S2 ~~ tr \<leadsto>* S3"
+    and no_i: "\<forall>a\<in>set tr. get_invoc a \<noteq> get_invoc ia"
+    and wf: "state_wellFormed S1"
+    and no_crash: "\<And>i. (i, ACrash) \<notin> set tr"
+    and no_endAtomic: "get_action ia \<noteq> AEndAtomic"
+    and no_endInvoc: "\<And>p. get_action ia \<noteq> AInvoc p"
+    and no_endReturn: "\<And>r. get_action ia \<noteq> AReturn r"
+    and a_no_crash: "get_action ia \<noteq> ACrash"
+  shows "\<exists>S3'. (S1 ~~ tr \<leadsto>* S3')" 
+proof -
+
+  obtain i a where ia_def[simp]: "ia = (i,a)"
+    by force
+  hence "i = get_invoc ia" and "a = get_action ia"
+    by auto
+
+  from step1 
+  have step: "S1 ~~ (i,a) \<leadsto> S2"
+    by simp
+
+  have wf2: "state_wellFormed S2"
+    using a_no_crash local.step local.wf state_wellFormed_combine_step  by fastforce
+
+  have no_i'[simp]: "i' \<noteq> i" if "(i', a) \<in> set tr" for i' a
+    using no_i that by auto
+  hence no_i''[simp]: "i \<noteq> i'" if "(i', a) \<in> set tr" for i' a
+    using that by blast
+
+  show ?thesis
+    using step
+  proof (cases rule: step.cases)
+    case (local ls f ok ls')
+
+    from steps 
+    have "S1 ~~ tr \<leadsto>* (S3\<lparr>localState := localState S3(i \<mapsto> ls)\<rparr>)"
+      using wf2 no_crash
+    proof (rule show_state_transfer2, goal_cases init step)
+      case init
+      thus ?case 
+        using local by (auto simp add: state_ext)
+    next
+      case (step i a Sa Sb)
+      thus ?case 
+        apply (cases a)
+        by (auto simp add: step.simps fun_upd_twist state_updates_normalize intro!: show_state_calls_eq ext)
+
+    qed
+    thus ?thesis
+      by blast
+
+
+  next
+    case (newId ls f ls' uid uidv ls'')
+    from steps 
+    have "S1 ~~ tr \<leadsto>* (S3\<lparr>localState := localState S3(i \<mapsto> ls), 
+                          generatedIds := (generatedIds S3)(uid := None)\<rparr>)"
+      using wf2 no_crash
+    proof (rule show_state_transfer2, goal_cases init step)
+      case init
+      thus ?case 
+        using newId by (auto simp add: state_ext)
+
+    next
+      case (step i' a Sa Sb)
+
+      have [simp]: "i' \<noteq> i" "i' \<noteq> i"
+        using ` (i', a) \<in> set tr` by auto
+
+      from newId
+      have "generatedIds S2 uid \<triangleq> i"
+        by auto
+
+      have [simp]: "uid \<noteq> to_nat x" if "a =  ANewId x" for x
+        using \<open>generatedIds S2 uid \<triangleq> i\<close> local.step(1) steps that uid_used_only_once by blast
+
+      from step
+      show ?case 
+        apply (cases a)
+        by (auto simp add: state_updates_normalize elim!: step_elims   intro!: stateEqI step_intros show_state_calls_eq ext)
+    qed
+    thus ?thesis by blast
+  next
+    case (beginAtomic ls f ls' t vis snapshot)
+
+    from steps 
+    have "S1 ~~ tr \<leadsto>* (S3\<lparr>
+                   localState := (localState S3)(i := localState S1 i),
+                   currentTransaction := (currentTransaction S3)(i := None),
+                   transactionStatus := (transactionStatus S3)(t := None),
+                   transactionOrigin := (transactionOrigin S3)(t := None),
+                   visibleCalls := (visibleCalls S3)(i := visibleCalls S1 i)\<rparr>)"
+      using wf2 no_crash
+    proof (rule show_state_transfer2, goal_cases init step)
+      case init
+      thus ?case 
+        using beginAtomic wf_transactionOrigin_and_status[OF wf] 
+        by (auto simp add: state_ext intro!: ext)
+    next
+      case (step i' a Sa Sb tr')
+
+      from no_i'
+      have tr'_no_i: "(i, a)\<notin>set tr'" for a
+        using `isPrefix tr' tr`
+        by (metis isPrefix_subset2)
+      have tr'_no_crash: "\<And>i. (i, ACrash) \<notin> set tr'"
+        by (meson isPrefix_subset2 local.step(4) no_crash)
+
+      
+
+      have monoGrowth: "state_monotonicGrowth i S2 Sa"
+      proof (auto simp add: state_monotonicGrowth_def `state_wellFormed S2` step intro!: exI[where x=tr'])
+        show "\<And>b. (i, b) \<in> set tr' \<Longrightarrow> False"
+          using \<open>\<And>a. (i, a) \<notin> set tr'\<close> by auto
+        show "\<And>i. (i, ACrash) \<in> set tr' \<Longrightarrow> False"
+          using \<open>\<And>i. (i, ACrash) \<notin> set tr'\<close> by blast
+      qed
+
+      have "state_wellFormed Sb"
+        using local.step(1) local.step(2) local.step(3) no_crash state_wellFormed_combine_step by fastforce
+
+      have "transactionStatus S2 t \<triangleq> Uncommitted"
+        using beginAtomic by simp
+
+      have "transactionStatus Sa t \<triangleq> Uncommitted"
+        by (smt \<open>transactionStatus S2 t \<triangleq> Uncommitted\<close> ia_def local.beginAtomic(7) local.step(3) local.wf monoGrowth option.distinct(1) state_monotonicGrowth_currentTransaction step1 unchangedInTransaction(3) wellFormed_currentTransaction_back4 wellFormed_currentTransaction_unique_h(2) wf2)
+
+
+
+      have [simp]: "tx' \<noteq> t" if "a = ABeginAtomic tx' txns'" for tx' txns'
+        using \<open>transactionStatus Sa t \<triangleq> Uncommitted\<close> local.step(2) step_elim_ABeginAtomic that by fastforce
+
+
+      have noCallsInTx_S2: "callOrigin S2 c \<noteq> Some t" for c
+        using beginAtomic wf_no_transactionStatus_origin_for_nothing[OF wf] by auto
+
+      have "currentTransaction S2 i \<triangleq> t"
+        by (smt currentTransaction_unchangedInternalSteps3 empty_iff ia_def list.set(1) local.beginAtomic(1) local.wf state_wellFormed_def step1 steps_append steps_step traceDeterministic)
+
+      have "currentTransaction Sa i \<triangleq> t"
+        using \<open>currentTransaction S2 i \<triangleq> t\<close> monoGrowth state_monotonicGrowth_currentTransaction by fastforce
+
+
+      have noCallsInTx: "callOrigin Sa c \<noteq> Some t" for c
+        using \<open>currentTransaction S2 i \<triangleq> t\<close> monoGrowth noCallsInTx_S2 state_monotonicGrowth_current_transactions_fixed by blast
+
+
+      show ?case 
+      proof (cases a)
+        case (ALocal x1)
+        with step show ?thesis by (auto simp add: step.simps fun_upd_twist state_updates_normalize intro!: show_state_calls_eq ext)
+      next
+        case (ANewId x2)
+        with step  show ?thesis by (auto simp add: step.simps fun_upd_twist state_updates_normalize intro!: show_state_calls_eq ext)
+      next
+        case (ABeginAtomic tx txns)
+        with step show ?thesis 
+          using \<open>transactionStatus Sa t \<triangleq> Uncommitted\<close> 
+          by (auto simp add: step.simps fun_upd_twist state_updates_normalize intro!: show_state_calls_eq ext elim!: chooseSnapshot_unchanged_precise)
+      next
+        case AEndAtomic
+        with step show ?thesis 
+          apply (auto simp add: step.simps fun_upd_twist state_updates_normalize intro!: show_state_calls_eq ext)
+          using \<open>currentTransaction Sa i \<triangleq> t\<close> no_i'' wellFormed_currentTransaction_unique by blast
+      next
+        case (ADbOp x51 x52 x53)
+        with step show ?thesis 
+          by (auto simp add: step.simps fun_upd_twist state_updates_normalize intro!: show_state_calls_eq ext)
+
+      next
+        case (AInvoc x6)
+        with step show ?thesis by (auto simp add: step.simps fun_upd_twist state_updates_normalize intro!: show_state_calls_eq ext)
+      next
+        case (AReturn x7)
+        with step show ?thesis by (auto simp add: step.simps fun_upd_twist state_updates_normalize intro!: show_state_calls_eq ext)
+      next
+        case ACrash
+        with step show ?thesis by (auto simp add: step.simps fun_upd_twist state_updates_normalize intro!: show_state_calls_eq ext)
+      next
+        case (AInvcheck ok)
+
+        have invContextSame: "(invContextH (callOrigin Sa) (\<lambda>a. if a = t then None else transactionOrigin Sa a)
+           (\<lambda>a. if a = t then None else transactionStatus Sa a) (happensBefore Sa) (calls Sa) (knownIds Sa) (invocationOp Sa)
+           (invocationRes Sa))
+          = invContext Sa"
+          using  step noCallsInTx
+          by (auto simp add: \<open>transactionStatus Sa t \<triangleq> Uncommitted\<close> AInvcheck step.simps  isCommittedH_def invContextH_def restrict_map_def restrict_relation_def committedCallsH_def intro!: ext, fastforce+)
+        from `a = AInvcheck ok` step show ?thesis 
+          by (auto simp add: invContextSame step.simps fun_upd_twist state_updates_normalize intro!: show_state_calls_eq ext)
+      qed
+    qed
+    thus ?thesis
+      by blast
+  next
+    case (endAtomic ls f ls' t)
+    show ?thesis
+      using `a = AEndAtomic` no_endAtomic by auto 
+  next
+    case (dbop ls f Op ls' t c res vis)
+    from steps 
+    have "S1 ~~ tr \<leadsto>* (S3\<lparr>
+                          localState := localState S3(i \<mapsto> ls), 
+                          calls := (calls S3)(c := None), 
+                          callOrigin := (callOrigin S3)(c := None),
+                          visibleCalls := visibleCalls S3(i \<mapsto> vis), 
+                          happensBefore := happensBefore S3 - vis \<times> {c}\<rparr>)"
+      using wf2 no_crash
+    proof (rule show_state_transfer2, goal_cases init step)
+      case init
+      thus ?case 
+        using dbop wellFormed_happensBefore_calls_r[OF wf] wellFormed_callOrigin_dom3[OF wf]
+        by (auto simp add:  intro!: ext stateEqI, blast)
+
+    next
+      case (step i' a Sa Sb  tr')
+
+      from no_i'
+      have tr'_no_i: "(i, a)\<notin>set tr'" for a
+        using `isPrefix tr' tr`
+        by (metis isPrefix_subset2)
+      have tr'_no_crash: "\<And>i. (i, ACrash) \<notin> set tr'"
+        by (meson isPrefix_subset2 local.step(4) no_crash)
+
+      
+
+      from `S2 ~~ tr' \<leadsto>* Sa` `state_wellFormed S2` `\<And>a. (i, a) \<notin> set tr'` `\<And>i. (i, ACrash) \<notin> set tr'`
+      have "state_monotonicGrowth i S2 Sa"
+        by (rule show_state_monotonicGrowth)
+
+      have "calls S2 c \<triangleq> Call Op res"
+        using dbop by auto
+
+      have "callOrigin S2 c \<triangleq> t"
+        using dbop by auto
+      have [simp]: "callOrigin Sa c \<triangleq> t"
+        using \<open>callOrigin S2 c \<triangleq> t\<close> \<open>state_monotonicGrowth i S2 Sa\<close> state_monotonicGrowth_callOrigin by blast 
+
+      have "currentTransaction S2 i \<triangleq> t"
+        using dbop by auto
+      hence "currentTransaction Sa i \<triangleq> t"
+        using \<open>state_monotonicGrowth i S2 Sa\<close> state_monotonicGrowth_currentTransaction by force
+
+
+      have "transactionStatus S2 t \<triangleq> Uncommitted"
+        using \<open>currentTransaction S2 i \<triangleq> t\<close> wellFormed_currentTransactionUncommitted wf2 by blast
+      have "transactionStatus Sa t \<triangleq> Uncommitted"
+        using \<open>currentTransaction Sa i \<triangleq> t\<close> local.step(3) wellFormed_currentTransactionUncommitted by blast
+
+
+
+      have [simp]: "calls Sa c \<triangleq> Call Op res"
+        using \<open>calls S2 c \<triangleq> Call Op res\<close> \<open>state_monotonicGrowth i S2 Sa\<close> state_monotonicGrowth_calls by blast
+
+      show ?case 
+      proof (cases a)
+        case (ALocal x1)
+        with step show ?thesis by (auto simp add: step.simps fun_upd_twist state_updates_normalize intro!: show_state_calls_eq ext)
+      next
+        case (ANewId x2)
+        with step show ?thesis by (auto simp add: step.simps fun_upd_twist state_updates_normalize intro!: show_state_calls_eq ext)
+      next
+        case (ABeginAtomic tx txns)
+
+        have h1: "callsInTransactionH (\<lambda>a. if a = c then None else callOrigin Sa a) newTxns \<down> (happensBefore Sa - vis \<times> {c})
+         =  callsInTransaction Sa newTxns \<down> happensBefore Sa" 
+          if " \<forall>txn\<in>newTxns. transactionStatus Sa txn \<triangleq> Committed"
+          for newTxns
+          using \<open>transactionStatus Sa t \<triangleq> Uncommitted\<close> not_uncommitted_cases that
+          apply (auto simp add: callsInTransactionH_def downwardsClosure_def)
+          using local.step(3) wellFormed_state_transaction_consistent(4) apply fastforce
+          by (metis (no_types, lifting) \<open>callOrigin Sa c \<triangleq> t\<close> option.inject)
+
+        from ABeginAtomic step 
+        show ?thesis apply (auto simp add: step.simps fun_upd_twist state_updates_normalize intro!: show_state_calls_eq ext)
+          apply (auto simp add: chooseSnapshot_h_def  )
+          subgoal for ls f ls' visa newTxns
+            apply (rule_tac x=newTxns in exI, auto)
+            apply (auto simp add: h1)
+            done
+          done
+
+      next
+        case AEndAtomic
+        with step show ?thesis by (auto simp add: step.simps fun_upd_twist state_updates_normalize intro!: show_state_calls_eq ext)
+      next
+        case (ADbOp c' op res)
+        with step show ?thesis 
+        proof (auto simp add: step.simps fun_upd_twist state_updates_normalize intro!: show_state_calls_eq ext, goal_cases)
+          case (1 ls f ls' t' vis')
+
+          have "getContextH (\<lambda>a. if a = c then None else calls Sa a) (happensBefore Sa - vis \<times> {c}) (Some vis')
+              = getContextH (calls Sa)                               (happensBefore Sa)             (Some vis')"
+            apply (auto simp add: getContextH_def restrict_map_def restrict_relation_def intro!: ext)
+            using "1"(13) \<open>currentTransaction Sa i \<triangleq> t\<close> \<open>transactionStatus Sa t \<triangleq> Uncommitted\<close> local.step(1) local.step(3) wellFormed_currentTransaction_unique wf_transactionConsistent1 apply fastforce
+            using "1"(13) \<open>currentTransaction Sa i \<triangleq> t\<close> \<open>transactionStatus Sa t \<triangleq> Uncommitted\<close> local.step(1) local.step(3) wellFormed_currentTransaction_unique wf_transactionConsistent1 by fastforce
+
+          with `querySpec (prog Sa) op (getContextH (calls Sa) (happensBefore Sa) (Some vis')) res`
+          show ?case by auto
+        qed
+
+      next
+        case (AInvoc x6)
+        with step show ?thesis by (auto simp add: step.simps fun_upd_twist state_updates_normalize intro!: show_state_calls_eq ext)
+      next
+        case (AReturn x7)
+        with step show ?thesis by (auto simp add: step.simps fun_upd_twist state_updates_normalize intro!: show_state_calls_eq ext)
+      next
+        case ACrash
+        with step show ?thesis by (auto simp add: step.simps fun_upd_twist state_updates_normalize intro!: show_state_calls_eq ext)
+      next
+        case (AInvcheck ok)
+        have invSame: "(invContextH (\<lambda>a. if a = c then None else callOrigin Sa a) (transactionOrigin Sa) (transactionStatus Sa)
+           (happensBefore Sa - vis \<times> {c}) (\<lambda>a. if a = c then None else calls Sa a) (knownIds Sa) (invocationOp Sa)
+           (invocationRes Sa))
+          = invContext Sa"
+          using   step 
+          using \<open>transactionStatus Sa t \<triangleq> Uncommitted\<close> 
+          by (auto simp add: wellFormed_callOrigin_dom2 AInvcheck step.simps  isCommittedH_def invContextH_def restrict_map_def restrict_relation_def committedCallsH_def intro!: ext)
+
+        with step show ?thesis 
+          by (auto simp add: AInvcheck invSame step.simps fun_upd_twist state_updates_normalize intro!: show_state_calls_eq ext)
+      qed
+
+
+    qed
+    thus ?thesis
+      by blast
+
+  next
+    case (invocation proc initialState impl)
+    then show ?thesis
+      using no_endInvoc \<open>a = get_action ia\<close> by metis
+  next
+    case (return ls f res)
+    then show ?thesis
+      using no_endReturn \<open>a = get_action ia\<close> by metis
+  next
+    case (fail ls)
+    then show ?thesis
+      using a_no_crash \<open>a = get_action ia\<close> by metis
+  next
+    case (invCheck res)
+    then show ?thesis
+      using steps by blast
+  qed
+qed
+
+(* 
+definition 
+"drop_no_action_coupling S1 S2 i \<equiv> 
+  calls S1 = calls S2
+\<and> happensBefore S1 = happensBefore S2
+\<and> callOrigin S1 = callOrigin S2
+\<and> (\<forall>t i'. i' \<noteq> i \<longrightarrow>  (transactionOrigin S1 t \<triangleq> i' \<longleftrightarrow> transactionOrigin S2 t \<triangleq> i'))
+\<and> (dom (transactionOrigin S2) \<subseteq> dom (transactionOrigin S1))
+\<and> knownIds S1 = knownIds S2
+\<and> invocationOp S1 = invocationOp S2
+\<and> invocationRes S1 = invocationRes S2
+\<and> prog S1 = prog S2
+\<and> (\<forall>t. currentTransaction S2 i \<noteq> Some t \<longrightarrow>  transactionStatus S1 t = transactionStatus S2 t)
+\<and> (\<forall>id i'. i' \<noteq> i \<longrightarrow> (generatedIds S1 id \<triangleq> i' \<longleftrightarrow> generatedIds S2 id \<triangleq> i'))
+\<and> (dom (generatedIds S2) \<subseteq> dom (generatedIds S1))
+\<and> (\<forall>i'. i' \<noteq> i \<longrightarrow> localState S1 i' = localState S2 i')
+\<and> currentProc S1 = currentProc S2
+\<and> (\<forall>i'. i' \<noteq> i \<longrightarrow> visibleCalls S1 i = visibleCalls S2 i)
+\<and> (\<forall>i'. i' \<noteq> i \<longrightarrow> currentTransaction S1 i = currentTransaction S2 i)
+"
+
+lemma drop_no_action:
+  assumes "S1 ~~ tr \<leadsto>* S1'"
+    and "\<forall>a\<in>set tr. get_invoc a \<noteq> i"
+    and "drop_no_action_coupling S1 S2 i"
+    and "state_wellFormed S1"
+    and "\<And>i. (i, ACrash) \<notin> set tr"
+  shows "\<exists>S2'. (S2 ~~ tr \<leadsto>* S2') \<and> drop_no_action_coupling S1' S2' i" 
+  using assms
+proof (induct rule: steps_induct)
+  case initial
+  then show ?case
+    using steps_empty by blast 
+
+next
+  case (step S' tr a S'')
+  obtain S2' where "S2 ~~ tr \<leadsto>* S2'" and coup: "drop_no_action_coupling S' S2' i"
+    using step.IH step.prems by auto
+
+  have not_i: "get_invoc a \<noteq> i"
+    by (simp add: step.prems(1))
+
+  have "state_wellFormed S'"
+    using state_wellFormed_combine step.prems step.steps by fastforce
+
+
+  from ` S' ~~ a \<leadsto> S''`
+  have "\<exists>S2''. (S2' ~~ a \<leadsto> S2'') \<and> drop_no_action_coupling S'' S2'' i"
+  proof (cases rule: step.cases)
+    case (local i ls f ok ls')
+    then show ?thesis 
+      using coup not_i by (auto simp add: step.simps  drop_no_action_coupling_def)
+  next
+    case (newId i ls f ls' uid uidv ls'')
+    then show ?thesis using coup not_i by (auto simp add: step.simps  drop_no_action_coupling_def)
+  next
+    case (beginAtomic i ls f ls' t vis snapshot)
+    then show ?thesis using coup not_i 
+      apply (auto simp add: step.simps  drop_no_action_coupling_def chooseSnapshot_unchanged)
+      
+      by (auto simp add: step.simps  drop_no_action_coupling_def chooseSnapshot_unchanged)
+  next
+    case (endAtomic i ls f ls' t)
+    then show ?thesis using coup not_i by (auto simp add: step.simps  drop_no_action_coupling_def)
+  next
+    case (dbop i ls f Op ls' t c res vis)
+    then show ?thesis using coup not_i by (auto simp add: step.simps  drop_no_action_coupling_def)
+  next
+    case (invocation i proc initialState impl)
+    then show ?thesis using coup not_i by (auto simp add: step.simps  drop_no_action_coupling_def)
+  next
+    case (return i ls f res)
+    then show ?thesis using coup not_i by (auto simp add: step.simps  drop_no_action_coupling_def)
+  next
+    case (fail i ls)
+    then show ?thesis using coup not_i by (auto simp add: step.simps  drop_no_action_coupling_def)
+  next
+    case (invCheck res i)
+    then show ?thesis using coup not_i by (auto simp add: step.simps  drop_no_action_coupling_def)
+  qed
+
+  then show ?case
+    using \<open>S2 ~~ tr \<leadsto>* S2'\<close> steps_step by blast 
+qed
+
+*)
+
+lemma steps_dropLast_tx:
+  assumes "S ~~ tr \<leadsto>* S'"
+    and "i < length tr"
+    and forbidden_actions: "get_action (tr!i) \<notin> {AEndAtomic} \<union> AReturn ` UNIV \<union> AInvoc ` UNIV"
+    and no_more_actions: "\<And>j. j>i \<Longrightarrow> j < length tr \<Longrightarrow> get_invoc (tr!j) \<noteq> get_invoc (tr!i)"
+    and wf: "state_wellFormed S"
+    and noCrash: "\<And>i. (i, ACrash) \<notin> set tr"
+  shows "\<exists>S''. S ~~ take i tr @ drop (Suc i) tr \<leadsto>* S''"
+proof -
+(*
+  have [simp]: "min (length tr) (i - Suc 0) = i - 1"
+    by (simp add: assms(3) less_imp_diff_less min_simps(2))
+
+  have [simp]: "i - Suc 0 + (length tr - i) = length tr - 1"
+    by (simp add: Suc_leI assms(2) assms(3) less_or_eq_imp_le)
+
+  have [simp]: "Suc (length tr - i) = Suc (length tr) - i"
+    by (simp add: Suc_diff_le assms(3) less_imp_le)
+
+
+  have [simp]: "length tr - (i - Suc 0) = Suc (length tr) - i"
+    using assms(2) assms(3) by auto
+
+  have [simp]: "Suc (length tr - Suc i) = length tr - i"
+    using Suc_diff_Suc assms(3) by blast
+*)
+
+  have "tr = take i tr @ drop i tr "
+    by (auto simp add: list_eq_iff_nth_eq nth_append nth_Cons')
+
+  moreover have "drop i tr = [tr!i] @ drop (Suc i) tr"
+    by (simp add: Cons_nth_drop_Suc assms(2))
+
+
+
+  ultimately have tr_split: "tr = take i tr @[tr!i] @ drop (Suc i) tr "
+    by simp
+
+  from this
+  obtain S1 S2 S3
+    where "S ~~ take i tr \<leadsto>* S1" and "S1 ~~ tr ! i \<leadsto> S2" and "S2 ~~ drop (Suc i) tr \<leadsto>* S3"
+    by (smt Cons_nth_drop_Suc \<open>drop i tr = [tr ! i] @ drop (Suc i) tr\<close> assms(1) assms(2) steps_append steps_appendFront)
+
+
+  thm drop_single_action
+  from `S1 ~~ tr ! i \<leadsto> S2` `S2 ~~ drop (Suc i) tr \<leadsto>* S3` 
+  have "\<exists>S3'. S1 ~~ drop (Suc i) tr \<leadsto>* S3'"
+  proof (rule drop_single_action)
+    from no_more_actions
+    show "\<forall>a\<in>set (drop (Suc i) tr). get_invoc a \<noteq> get_invoc (tr ! i)"
+      by (auto simp add: in_set_conv_nth, 
+          metis add.commute add_Suc_right fst_conv less_add_Suc1 less_diff_conv)
+    show "state_wellFormed S1"
+      by (meson \<open>S ~~ take i tr \<leadsto>* S1\<close> local.wf noCrash set_take_subset state_wellFormed_combine subsetD)
+    show "\<And>ia. (ia, ACrash) \<notin> set (drop (Suc i) tr)"
+      by (meson in_set_dropD noCrash)
+    show "get_action (tr ! i) \<noteq> AEndAtomic"
+      using forbidden_actions by blast
+    show "\<And>p. get_action (tr ! i) \<noteq> AInvoc p"
+      using assms(3) by blast
+    show "\<And>r. get_action (tr ! i) \<noteq> AReturn r"
+      using forbidden_actions by blast
+    show "get_action (tr ! i) \<noteq> ACrash"
+      by (metis assms(2) noCrash nth_mem prod.collapse)
+  qed
+  from this obtain S3' where "S1 ~~ drop (Suc i) tr \<leadsto>* S3'"
+    by blast
+
+
+  from `S ~~ take i tr \<leadsto>* S1` and `S1 ~~ drop (Suc i) tr \<leadsto>* S3'`
+  show ?thesis
+    using steps_append2 by blast
+qed
+
+lemma no_return_in_transaction:
+  assumes "S ~~ tr \<leadsto>* S_end"
+    and "tr ! i_start = (invoc, ABeginAtomic tx txns)"
+    and no_end_atomic: "\<And>j. \<lbrakk>i_start < j \<and> j \<le> i_r\<rbrakk> \<Longrightarrow> tr ! j \<noteq> (invoc, AEndAtomic)"
+    and "i_start \<le> i_r"
+    and "i_r < length tr"
+    and "state_wellFormed S"
+    and noCrash: "\<And>i. (i, ACrash) \<notin> set tr"
+  shows "tr ! i_r \<noteq> (invoc, AReturn r)" and "\<And>S'. (S ~~ take (Suc i_r) tr \<leadsto>* S') \<Longrightarrow> currentTransaction S' invoc \<triangleq> tx"
+proof -
+
+  from `i_start \<le> i_r` and `i_r < length tr` and no_end_atomic
+  have " tr ! i_r \<noteq> (invoc, AReturn r) \<and> (\<forall>S'. (S ~~ take (Suc i_r) tr \<leadsto>* S') \<longrightarrow> currentTransaction S' invoc \<triangleq> tx)"
+  proof (induct "i_r - i_start" arbitrary: i_r)
+    case (0 i_r)
+    hence "i_r = i_start"
+      by linarith
+
+
+    show ?case 
+    proof (intro allI impI conjI)
+
+
+      show "currentTransaction S' invoc \<triangleq> tx"
+        if c0: "S ~~ take (Suc i_r) tr \<leadsto>* S'"
+        for  S'
+      proof -
+
+
+        from `S ~~ take (Suc i_r) tr \<leadsto>* S'`
+        obtain S_pre where "S ~~ take i_start tr \<leadsto>* S_pre" and "S_pre ~~ tr ! i_start \<leadsto> S'"
+          by (metis "0.prems"(2)  \<open>i_r = i_start\<close>  steps_appendBack take_Suc_conv_app_nth)
+
+        from `S_pre ~~ tr ! i_start \<leadsto> S'` 
+          and `tr ! i_start = (invoc, ABeginAtomic tx txns)`
+        show "currentTransaction S' invoc \<triangleq> tx" 
+          by (auto simp add: step.simps)
+      qed
+
+      show "tr ! i_r \<noteq> (invoc, AReturn r)"
+        by (simp add: \<open>i_r = i_start\<close> assms(2))
+    qed
+  next
+    case (Suc x)
+
+    have IH: "tr ! (i_r - 1) \<noteq> (invoc, AReturn r) \<and> (\<forall>S'. (S ~~ take (Suc (i_r - 1)) tr \<leadsto>* S') \<longrightarrow> currentTransaction S' invoc \<triangleq> tx)"
+    proof (rule Suc.hyps)
+      show "x = i_r - 1 - i_start"
+        using Suc.hyps(2) by auto
+      show "i_start \<le> i_r - 1"
+        using Suc.hyps(2) by auto
+      show "i_r - 1 < length tr"
+        using Suc.prems(2) less_imp_diff_less by blast
+      show "\<And>j. i_start < j \<and> j \<le> i_r - 1 \<Longrightarrow> tr ! j \<noteq> (invoc, AEndAtomic)"
+        using Suc.prems(3) by force
+    qed
+    hence ctx: "currentTransaction S' invoc \<triangleq> tx" if "S ~~ take i_r tr \<leadsto>* S'" for S'
+      using that `Suc x = i_r - i_start` by force 
+
+    have noEndAtomic: "tr ! i_r \<noteq> (invoc, AEndAtomic)"
+      using Suc.hyps(2) Suc.prems(3) by auto
+
+
+    obtain  S' S'' where "S ~~ take i_r tr \<leadsto>* S'" and "S' ~~ tr ! i_r \<leadsto> S''"
+      by (metis Suc.prems(2) assms(1) id_take_nth_drop steps_append steps_appendFront)
+
+
+    moreover {
+      fix  S' S'' 
+      assume "S ~~ take i_r tr \<leadsto>* S'" and "S' ~~ tr ! i_r \<leadsto> S''"
+
+      have "currentTransaction S' invoc \<triangleq> tx"
+        using \<open>S ~~ take i_r tr \<leadsto>* S'\<close> ctx by blast
+
+      with `S' ~~ tr ! i_r \<leadsto> S''` noEndAtomic
+      have "currentTransaction S'' invoc \<triangleq> tx" and "tr ! i_r \<noteq> (invoc, AReturn r)"
+         apply (auto simp add: step.simps)
+        using Suc.prems(2) noCrash nth_mem by fastforce
+    }
+    ultimately show ?case
+      by (metis Suc.prems(2) steps_step take_Suc_conv_app_nth traceDeterministic)
+  qed
+  thus "tr ! i_r \<noteq> (invoc, AReturn r)"
+    and "\<And>S'. S ~~ take (Suc i_r) tr \<leadsto>* S' \<Longrightarrow> currentTransaction S' invoc \<triangleq> tx"
+    by auto
+qed
+
+
+
+
 
 definition "induct_measure" where "induct_measure  \<equiv> \<lambda>trace. \<lambda>pos'.
     case pos' of
         0 \<Rightarrow> True
       | Suc pos \<Rightarrow>  pos<length trace \<and> (\<exists>i j tx txns. get_invoc(trace!pos) = i \<and>  j\<le>pos \<and> trace!j = (i, ABeginAtomic tx txns) \<and> (\<nexists>k. k>j \<and> k<length trace \<and> trace!k = (i, AEndAtomic)))" 
 
-
 text \<open>
- To show that a program is correct, we only have to consider packed and finished transactions
+ To show that a program is correct, we only have to consider packed traces
+with no context switches in transactions.
 \<close>
-theorem show_programCorrect_noTransactionInterleaving'':
-  assumes packedTracesCorrect: 
-    "\<And>trace s. \<lbrakk>
-      initialState program ~~ trace \<leadsto>* s; 
-      packed_trace trace; 
-      allTransactionsEnd trace;  
-      \<And>s. (s, ACrash) \<notin> set trace; 
-      no_invariant_checks_in_transaction trace
-    \<rbrakk> \<Longrightarrow> traceCorrect trace"
-  shows "programCorrect program"
-proof (rule show_programCorrect_noTransactionInterleaving')
-  fix trace 
-  fix s
-  assume steps: "initialState program ~~ trace \<leadsto>* s"
-    and packed: "packed_trace trace" 
-    and nofail: "\<And>s. (s, ACrash) \<notin> set trace"
-    and no_inv_checks: "no_invariant_checks_in_transaction trace"
+lemma remove_context_switches_in_transactions:
+  assumes a1: "initialState program ~~ trace \<leadsto>* S"
+    and a2: "packed_trace trace"
+    and a3: "\<And>s. (s, ACrash) \<notin> set trace"
+    and a4: "\<And>s. (s, AInvcheck True) \<notin> set trace"
+    and a5: "no_invariant_checks_in_transaction trace"
+    and a6: "\<not>traceCorrect trace"
+  obtains trace' S'
+  where "initialState program ~~ trace' \<leadsto>* S'"
+    and "packed_trace trace'"
+    and "\<And>s. (s, ACrash) \<notin> set trace'"
+    and "\<And>s. (s, AInvcheck True) \<notin> set trace'"
+    and "no_invariant_checks_in_transaction trace'"
+    and "\<not>traceCorrect trace'"
+    and "\<not>contextSwitchesInTransaction trace'"
+  using a1 a2 a3 a4 a5 a6 proof (atomize_elim, induct "length trace" arbitrary: S trace rule: less_induct)
+  case (less trace S)
+
+  show ?case
+  proof (rule classical, goal_cases trivial)
+    case trivial
+
+    hence trivial1: "(\<not>P \<Longrightarrow> ?case) \<Longrightarrow> P" for P
+      by blast
+
+    hence trivial2: "(P \<Longrightarrow> ?case) \<Longrightarrow> \<not>P" for P
+      by blast
+
+    have all_actions_correct_but_last: "actionCorrect (get_action a)" if "trace ! i = a" and "i < length trace - 1" for i a
+    proof (rule trivial1)
+      assume "\<not> actionCorrect (get_action a)"
+
+      have len: "length (take (Suc i) trace) < length trace"
+        using that(2) by auto
+
+
+      obtain S' where steps': "initialState program ~~ take (Suc i) trace \<leadsto>* S'"
+        by (metis append_take_drop_id less.prems(1) steps_append)
+
+
+      show ?case 
+        using len steps'
+      proof (rule less)
+        show "packed_trace (take (Suc i) trace)"
+          using less.prems(2) packed_trace_take by blast
+        show "\<And>s. (s, ACrash) \<notin> set (take (Suc i) trace)"
+          by (meson in_set_takeD less.prems(3))
+        show "\<And>s. (s, AInvcheck True) \<notin> set (take (Suc i) trace)"
+          by (meson in_set_takeD less.prems(4))
+        show "no_invariant_checks_in_transaction (take (Suc i) trace)"
+          by (metis append_take_drop_id isPrefix_appendI less.prems(5) no_invariant_checks_in_transaction_prefix)
+        show "\<not> traceCorrect (take (Suc i) trace)"
+          by (metis (no_types, lifting) \<open>\<not> actionCorrect (get_action a)\<close> len length_take lessI min_less_iff_conj min_simps(2) nat_neq_iff nth_append_length nth_mem take_Suc_conv_app_nth that(1) traceCorrect_def)
+        show "initialState program ~~ take (Suc i) trace \<leadsto>* S'"
+          using steps' by blast
+        show "packed_trace (take (Suc i) trace)"
+          by (simp add: \<open>packed_trace (take (Suc i) trace)\<close>)
+        show "\<And>s. (s, ACrash) \<notin> set (take (Suc i) trace)"
+          using \<open>\<And>s. (s, ACrash) \<notin> set (take (Suc i) trace)\<close> by blast
+        show "\<And>s. (s, AInvcheck True) \<notin> set (take (Suc i) trace)"
+          by (simp add: \<open>\<And>s. (s, AInvcheck True) \<notin> set (take (Suc i) trace)\<close>)
+        show "no_invariant_checks_in_transaction (take (Suc i) trace)"
+          by (simp add: \<open>no_invariant_checks_in_transaction (take (Suc i) trace)\<close>)
+        show "\<not> traceCorrect (take (Suc i) trace)"
+          by (simp add: \<open>\<not> traceCorrect (take (Suc i) trace)\<close>)
+      qed
+    qed
+
+    hence last_action_incorrect: "\<not>actionCorrect (get_action (last trace))"
+      by (metis (no_types, lifting) append_butlast_last_id in_set_conv_nth last_conv_nth length_append_singleton length_butlast length_pos_if_in_set less.prems(6) less_antisym less_numeral_extra(3) list.size(3) traceCorrect_def)
+
+
+    have "contextSwitchesInTransaction trace"
+    proof (rule trivial1)
+      assume "\<not>contextSwitchesInTransaction trace"
+      thus ?case
+        using less by blast
+    qed
+
+    from this obtain i_begin1 i_switch1
+      where "contextSwitchInTransaction trace i_begin1 i_switch1"
+      by (auto simp add: contextSwitchesInTransaction_def)
+
+    from this obtain i_begin i_switch
+      where i_switch: "contextSwitchInTransaction trace i_begin i_switch"
+        and i_switch_min: "\<And>i_begin' i_switch'. contextSwitchInTransaction trace i_begin' i_switch' \<Longrightarrow> i_switch \<le> i_switch'"
+      using exists_min_wellorder[where P="\<lambda>i_switch. \<exists>i_begin. contextSwitchInTransaction trace i_begin i_switch"]
+      by meson
+
+    from i_switch_min
+    have no_earlier_context_switches:
+       "\<And>j. \<lbrakk>i_begin < j; j < i_switch\<rbrakk> \<Longrightarrow> \<not> allowed_context_switch (get_action (trace ! j))"
+      using i_switch_min      by (smt contextSwitchInTransaction_def dual_order.strict_trans i_switch leD)
+
+
+    from i_switch
+    obtain invoc tx txns
+      where a0: "i_begin < i_switch"
+        and a1: "i_switch < length trace"
+        and a2: "trace ! i_begin = (invoc, ABeginAtomic tx txns)"
+        and a3: "\<forall>j. i_begin < j \<and> j < i_switch \<longrightarrow> trace ! j \<noteq> (invoc, AEndAtomic)"
+        and a4: "allowed_context_switch (get_action (trace ! i_switch))"
+      by (auto simp add: contextSwitchInTransaction_def)
+
+    have same_invoc:
+      "get_invoc (trace ! j) = invoc" if "i_begin \<le> j" and "j < i_switch" for j
+      using `initialState program ~~ trace \<leadsto>* S`
+        `trace ! i_begin = (invoc, ABeginAtomic tx txns)`
+    proof (rule no_context_switch_transaction2)
+      show "\<And>ja. \<lbrakk>i_begin < ja; ja \<le> j\<rbrakk> \<Longrightarrow> trace ! ja \<noteq> (invoc, AEndAtomic)"
+        using a3 order.strict_trans1 that(2) by blast
+      from `packed_trace trace`
+      show "packed_trace trace" .
+
+      show "\<And>ja. \<lbrakk>i_begin < ja; ja \<le> j\<rbrakk> \<Longrightarrow> \<not> allowed_context_switch (get_action (trace ! ja))"
+        by (simp add: le_less_trans no_earlier_context_switches that(2))
+      show "i_begin \<le> j"
+        by (simp add: that(1))
+      show "j < length trace"
+        using a1 dual_order.strict_trans that(2) by blast
+    qed
+
+
+    text "We are in a transaction, so execution up to j gives 
+  us a state with a current transaction:"
+    obtain S_j_pre
+      where "initialState program ~~ take i_switch trace \<leadsto>* S_j_pre"
+      by (metis a1 id_take_nth_drop less.prems(1) steps_append)
+
+
+    from this
+    have "currentTransaction S_j_pre invoc \<triangleq> tx"
+    proof (rule currentTransaction2)
+      show "i_begin < length (take i_switch trace)"
+        by (simp add: a0 a1 min_simps(2))
+      show " take i_switch trace ! i_begin = (invoc, ABeginAtomic tx txns)"
+        by (simp add: a0 a2) 
+      fix ja
+      assume a0: "i_begin < ja"
+        and a1: "ja < length (take i_switch trace)"
+
+      show "take i_switch trace ! ja \<noteq> (invoc, ACrash)"
+        using a1 less.prems(3) nth_mem by fastforce
+
+      show "take i_switch trace ! ja \<noteq> (invoc, AEndAtomic)"
+        using a0 a1 a3 by auto
+    qed
+
+    have "state_wellFormed S_j_pre"
+      by (meson \<open>initialState program ~~ take i_switch trace \<leadsto>* S_j_pre\<close> less.prems(3) set_take_subset state_wellFormed_combine state_wellFormed_init subsetD)
+
+    have "i_switch < length trace"
+      by (simp add: a1)
 
 
 
-  have induct_measure_ex: "\<exists>x. induct_measure trace x" for trace
-    by (rule exI[where x=0], auto simp add: induct_measure_def)
+    obtain S_j_post
+      where "S_j_pre ~~ trace ! i_switch \<leadsto> S_j_post"
+      by (metis (no_types, lifting) \<open>initialState program ~~ take i_switch trace \<leadsto>* S_j_pre\<close> a1 id_take_nth_drop less.prems(1) steps_append2 steps_appendFront)
 
-  have induct_measure_bound: "\<exists>bound. \<forall>x. induct_measure trace x \<longrightarrow> x \<le> bound" for trace
-    by (rule exI[where x="length trace"], auto simp add: induct_measure_def split: nat.split)
 
-  from steps packed nofail no_inv_checks
-  show "traceCorrect trace"
-  proof (induct "GREATEST pos'. induct_measure trace pos'"
-      arbitrary: trace s rule: less_induct)
-    case (less trace')
-    show ?case
-    proof (cases "Greatest (induct_measure trace')")
-      case (0)
-      then have [simp]: "(GREATEST a. induct_measure trace' a) = 0" by simp
-      have "induct_measure trace' (GREATEST x. induct_measure trace' x) \<and> (\<forall>y. induct_measure trace' y \<longrightarrow> y \<le> (GREATEST x. induct_measure trace' x))"
-        by (rule use_Greatest[OF induct_measure_ex induct_measure_bound])
-      then have "\<nexists>pos. pos < length trace' \<and>
-                         (\<exists>i j tx txns. get_invoc (trace' ! pos) = i \<and> j \<le> pos \<and> trace' ! j = (i, ABeginAtomic tx txns) \<and> \<not> (\<exists>k>j. k < length trace' \<and> trace' ! k = (i, AEndAtomic)))"
-        by (simp, auto simp add: induct_measure_def split: nat.splits)
-      then have "allTransactionsEnd trace'"
-        by (auto simp add: allTransactionsEnd_def, force)
-      then show "traceCorrect trace'"
-        using "less.prems" packedTracesCorrect by blast
+
+    text "Since we are in a transaction, the action at position j cannot be a
+  context switch on the same invocation"
+
+    with `allowed_context_switch (get_action (trace ! i_switch))`
+      and `currentTransaction S_j_pre invoc \<triangleq> tx`
+    have "get_invoc (trace ! i_switch) \<noteq> invoc"
+      using  inTransaction_localState[OF \<open>state_wellFormed S_j_pre\<close>] 
+      by (auto simp add: step.simps, blast)
+
+    have "i_switch < length trace"
+      by (simp add: a1)
+
+    have "i_switch > 0"
+      using a0 by linarith
+
+
+    have "S_j_pre ~~ drop i_switch trace \<leadsto>* S"
+      using \<open>initialState program ~~ take i_switch trace \<leadsto>* S_j_pre\<close> less.prems(1) steps_append2 by fastforce
+
+    from this
+    have "currentTransaction S invoc \<triangleq> tx \<and> (\<forall>a\<in>set (drop i_switch trace). get_invoc a \<noteq> invoc)"
+    proof (rule no_more_actions_on_packed_trace_if_context_switch_in_transaction)
+      show "packed_trace (drop i_switch trace)"
+        by (simp add: less.prems(2) packed_trace_drop)
+      show "currentTransaction S_j_pre invoc \<triangleq> tx"
+        by (simp add: \<open>currentTransaction S_j_pre invoc \<triangleq> tx\<close>)
+      show "get_invoc (hd (drop i_switch trace)) \<noteq> invoc"
+        by (simp add: \<open>get_invoc (trace ! i_switch) \<noteq> invoc\<close> \<open>i_switch < length trace\<close> hd_drop_conv_nth)
+      show "drop i_switch trace \<noteq> []"
+        using \<open>i_switch < length trace\<close> drop_eq_Nil leD by blast
+      show "state_wellFormed S_j_pre"
+        by (simp add: \<open>state_wellFormed S_j_pre\<close>)
+      show "\<And>i. (i, ACrash) \<notin> set (drop i_switch trace)"
+        by (meson in_set_dropD less.prems(3))
+    qed
+
+
+    hence "get_invoc (trace ! j') \<noteq> invoc" if "j' > i_switch" and "j' < length trace" for j'
+      using that apply (auto simp add: all_set_conv_all_nth)
+      by (metis diff_less_mono less_or_eq_imp_le ordered_cancel_comm_monoid_diff_class.add_diff_inverse)
+
+
+    show ?thesis
+    proof (cases "get_action (trace ! (i_switch - 1)) = ALocal False")
+      case True
+      text "If the action before j was a context, then only consider the trace up to this and use IH."
+
+      thm less.hyps
+
+      have "isPrefix (take i_switch trace) trace"
+        by (metis append_take_drop_id isPrefix_appendI)
+
+
+      show ?thesis
+      proof (rule less.hyps)
+        show "length (take i_switch trace) < length trace"
+          using \<open>i_switch < length trace\<close> by auto
+        show "initialState program ~~ take i_switch trace \<leadsto>* S_j_pre"
+          using \<open>initialState program ~~ take i_switch trace \<leadsto>* S_j_pre\<close> by blast
+        show "packed_trace (take i_switch trace)"
+          using less.prems(2) packed_trace_take by blast
+        show "\<And>s. (s, ACrash) \<notin> set (take i_switch trace)"
+          by (meson in_set_takeD less.prems(3))
+        show "no_invariant_checks_in_transaction (take i_switch trace)"
+          using `no_invariant_checks_in_transaction trace`
+          using \<open>isPrefix (take i_switch trace) trace\<close> no_invariant_checks_in_transaction_prefix by blast
+        show "\<not> traceCorrect (take i_switch trace)"
+        proof (auto simp add: traceCorrect_def, intro bexI)
+          show "(trace ! (i_switch - 1)) \<in> set (take i_switch trace) "
+            by (metis \<open>0 < i_switch\<close> a1 diff_less length_take min_simps(2) nth_mem nth_take zero_less_one)
+          show "\<not> actionCorrect (get_action (trace ! (i_switch - 1)))"
+            using True actionCorrect_def by blast
+        qed
+        show "initialState program ~~ take i_switch trace \<leadsto>* S_j_pre"
+          using \<open>initialState program ~~ take i_switch trace \<leadsto>* S_j_pre\<close> by auto
+        show "packed_trace (take i_switch trace)"
+          using \<open>packed_trace (take i_switch trace)\<close> by blast
+        show "\<And>s. (s, ACrash) \<notin> set (take i_switch trace)"
+          using \<open>\<And>s. (s, ACrash) \<notin> set (take i_switch trace)\<close> by blast
+        show "no_invariant_checks_in_transaction (take i_switch trace)"
+          using \<open>no_invariant_checks_in_transaction (take i_switch trace)\<close> by blast
+        show "\<not> traceCorrect (take i_switch trace)"
+          by (simp add: \<open>\<not> traceCorrect (take i_switch trace)\<close>)
+        show "\<And>s. (s, AInvcheck True) \<notin> set (take i_switch trace)"
+          by (meson in_set_takeD less.prems(4))
+        thus "\<And>s. (s, AInvcheck True) \<notin> set (take i_switch trace)" .
+      qed
+
     next
-      case (Suc pos )
-      then have [simp]: "(GREATEST x. induct_measure trace' x) = Suc pos" by simp
+      case False
 
-      have "induct_measure trace' (GREATEST x. induct_measure trace' x) \<and> (\<forall>y. induct_measure trace' y \<longrightarrow> y \<le> (GREATEST x. induct_measure trace' x))"
-        by (rule use_Greatest[OF induct_measure_ex induct_measure_bound])
-      then have m: "induct_measure trace' (Suc pos)"
-        and  m_max: "induct_measure trace' y \<Longrightarrow> y \<le> Suc pos" for y
-        by auto
+      text "Otherwise, remove the action"
 
-      from m have "pos<length trace' \<and> (\<exists>i j tx txns. get_invoc(trace'!pos) = i \<and>  j\<le>pos \<and> trace'!j = (i, ABeginAtomic tx txns) \<and> (\<nexists>k. k>j \<and> k<length trace' \<and> trace'!k = (i, AEndAtomic)))"
-        by (auto simp add: induct_measure_def split: nat.splits)
-      from this obtain j tx txns
-        where pos_less: "pos < length trace'"
-          and j_leq_pos: "j \<le> pos"
-          and noEndAtomic_trace': "\<forall>k<length trace'. j < k \<longrightarrow> trace' ! k \<noteq> (get_invoc (trace' ! pos), AEndAtomic)"
-          and beginAtomic_trace': "trace' ! j = (get_invoc (trace' ! pos), ABeginAtomic tx txns)"
-        by auto
-
-      have maxPos: "get_invoc (trace'!pos') \<noteq> get_invoc(trace'!pos)" if "pos' > pos" and "pos' < length trace'" for pos'
-        using m_max[where y2="Suc pos'"] that
-          beginAtomic_trace' j_leq_pos le_less_trans less_imp_le noEndAtomic_trace'
-          by (auto simp add: induct_measure_def, blast )
+      define trace' where "trace' = take (i_switch - 1) trace @ drop i_switch trace"
 
 
 
-\<comment> \<open>get new trace by removing action at pos\<close>
-      define newTrace where "newTrace = take pos trace' @ drop (Suc pos) trace'"
-
-      have newTraceLen: "length newTrace = length trace' - 1"
-        using \<open>pos < length trace'\<close> newTrace_def by auto
-
-      have [simp]: "min (length trace') pos = pos"
-        using \<open>pos < length trace'\<close> by auto
+      have "length trace = Suc (length trace')"
+        using \<open>0 < i_switch\<close> \<open>i_switch < length trace\<close> trace'_def by auto
 
 
-      have newTraceIth: "newTrace!i = (if i<pos then trace'!i else trace'!Suc i)" if "i<length newTrace"  for i
-        using that \<open>pos < length trace'\<close> by (auto simp add: newTrace_def nth_append)
+      obtain S' where 
+        " initialState program ~~ trace' \<leadsto>* S'"
+        unfolding trace'_def
 
-      have IH: " \<lbrakk>Greatest (induct_measure trace) < Greatest (induct_measure trace'); \<exists>S. initialState program ~~ trace \<leadsto>* S; packed_trace trace; \<And>s. (s, ACrash) \<notin> set trace; no_invariant_checks_in_transaction trace\<rbrakk>
-     \<Longrightarrow> traceCorrect trace" for trace
-        using less.hyps   by auto 
+      proof (atomize_elim, fuzzy_rule steps_dropLast_tx)
+        show "initialState program ~~ trace \<leadsto>* S"
+          by (simp add: less.prems(1))
+        show " get_action (trace ! (i_switch - 1)) \<notin> {AEndAtomic} \<union> range AReturn \<union> range AInvoc" (is ?goal)
+proof auto
+            text "It cannot be any of these cases, because we are in an unfinished transaction ..."
 
 
-      have "traceCorrect newTrace"
-      proof (rule IH, simp)
-        show "Greatest (induct_measure newTrace) < Suc pos"
-        proof (rule Greatest_smaller[OF induct_measure_ex induct_measure_bound])
-          fix y
-          assume a0: "induct_measure newTrace y"
-          {
-            assume "y > 0" and "y > pos"
+            have "i_switch - Suc 0 < i_switch"
+              using \<open>0 < i_switch\<close> diff_Suc_less by blast
 
-            with a0 obtain j tx txns
-              where a1: "y < Suc (length newTrace)" 
-                and a2: "j < y"
-                and a3: "\<forall>k<length newTrace. j < k \<longrightarrow> newTrace ! k \<noteq> (get_invoc (newTrace ! (y-1)), AEndAtomic)"
-                and a4: "newTrace ! j = (get_invoc (newTrace ! (y-1)), ABeginAtomic tx txns)"
-              using le_imp_less_Suc by (auto simp add: induct_measure_def split: nat.splits, blast)
+            have "i_begin \<le> i_switch - Suc 0"
+              using a0 by linarith
 
-            have [simp]: "j < length newTrace"
-              using a1 a2 by linarith
 
-            have [simp]: "y - Suc 0 < length newTrace"
-              using \<open>0 < y\<close> a1 by linarith
+            have "trace ! (i_switch - Suc 0) \<noteq> (invoc, AEndAtomic)"
+              by (metis \<open>i_begin \<le> i_switch - Suc 0\<close> \<open>i_switch - Suc 0 < i_switch\<close> a2 a3 action.distinct(31) le_neq_implies_less old.prod.inject)
 
-            have [simp]: " \<not>(y - Suc 0 < pos)"
-              using \<open>pos < y\<close> by linarith
 
-            have [simp]: "Suc (y - Suc 0) = y"
-              by (simp add: \<open>0 < y\<close>)
+            have "get_invoc (trace ! (i_switch - Suc 0)) = invoc"
+              using a0 same_invoc by auto
 
-            from a4 have a4': "newTrace ! j = (get_invoc (trace' ! y), ABeginAtomic tx txns)"
-              by (simp add: newTraceIth)
 
-            have [simp]: "y < length trace'"
-              using \<open>pos < length trace'\<close> a1 newTraceLen by linarith
+            show "get_action (trace ! (i_switch - Suc 0)) = AEndAtomic \<Longrightarrow> False"
+              by (metis \<open>get_invoc (trace ! (i_switch - Suc 0)) = invoc\<close> \<open>trace ! (i_switch - Suc 0) \<noteq> (invoc, AEndAtomic)\<close> surjective_pairing)
 
-            have "induct_measure trace' (Suc y)"
-              using a4 a3
-            proof (auto simp add: induct_measure_def newTraceIth split: if_splits)
-              show "\<exists>j\<le>y. (\<exists>tx txns. trace' ! j = (get_invoc (trace' ! y), ABeginAtomic tx txns)) \<and> (\<forall>k<length trace'. j < k \<longrightarrow> trace' ! k \<noteq> (get_invoc (trace' ! y), AEndAtomic))" 
-                if c1: "\<forall>k. (j < k \<longrightarrow> k < length newTrace \<longrightarrow> k < pos \<longrightarrow> trace' ! k \<noteq> (get_invoc (trace' ! y), AEndAtomic)) 
-                      \<and> (j < k \<longrightarrow> k < length newTrace \<longrightarrow> k < pos \<or> trace' ! Suc k \<noteq> (get_invoc (trace' ! y), AEndAtomic))"
-                  and c2: "j < pos" 
-                  and c3: "trace' ! j = (get_invoc (trace' ! y), ABeginAtomic tx txns)"
-              proof (rule exI[where x=j], auto simp add: c3)
-                show "j \<le> y"
-                  using a2 by linarith
-                show "False" 
-                  if "k < length trace'" 
-                    and "j < k" 
-                    and "trace' ! k = (get_invoc (trace' ! y), AEndAtomic)" for k
-                proof (cases "k < pos")
-                  case True
-                  with c1 have "trace' ! k \<noteq> (get_invoc (trace' ! y), AEndAtomic)"
-                    using \<open>pos < y\<close> a1 that(2) by auto
-                  then show False
-                    using that(3) by blast
-                next
-                  case False
-                  with c1[rule_format, where k="k - 1"]
-                  have "trace' ! k \<noteq> (get_invoc (trace' ! y), AEndAtomic)"
-                    by (smt One_nat_def Suc_pred \<open>pos < y\<close> \<open>y < length trace'\<close> c2 fst_conv less_Suc_eq maxPos newTraceLen not_less0 not_less_iff_gr_or_eq that(1) that(2))
-                  then show False
-                    using that(3) by blast
-                qed
-              qed
-              show "\<exists>j\<le>y. (\<exists>tx txns. trace' ! j = (get_invoc (trace' ! y), ABeginAtomic tx txns)) \<and> (\<forall>k<length trace'. j < k \<longrightarrow> trace' ! k \<noteq> (get_invoc (trace' ! y), AEndAtomic))"
-                if c1: "\<forall>k<length newTrace. j < k \<longrightarrow> trace' ! Suc k \<noteq> (get_invoc (trace' ! y), AEndAtomic)"
-                  and c2: "\<not> j < pos"
-                  and c3: "trace' ! Suc j = (get_invoc (trace' ! y), ABeginAtomic tx txns)"
-              proof (rule exI[where x="Suc j"], auto simp add: c3)
-                show "Suc j \<le> y"
-                  using a2 by auto
-                show "False" if "k < length trace'"
-                  and "Suc j < k"
-                  and "trace' ! k = (get_invoc (trace' ! y), AEndAtomic)"
-                for k
-                proof -
-                  from c1[rule_format, where k="k-1"]
-                  have "trace' ! k \<noteq> (get_invoc (trace' ! y), AEndAtomic)"
-                    by (metis One_nat_def Suc_less_eq Suc_pred linorder_neqE_nat newTraceLen not_less0 that(1) that(2))
-                  then show False
-                    using that(3) by linarith
+            show "\<And>x. get_action (trace ! (i_switch - Suc 0)) = AReturn x \<Longrightarrow> False"
+              using no_return_in_transaction(1)[OF `initialState program ~~ trace \<leadsto>* S` `trace ! i_begin = (invoc, ABeginAtomic tx txns)`, where i_r="i_switch - Suc 0"]
+              by (metis (no_types, lifting) \<open>get_invoc (trace ! (i_switch - Suc 0)) = invoc\<close> \<open>i_begin \<le> i_switch - Suc 0\<close> \<open>i_switch - Suc 0 < i_switch\<close> a1 a3 dual_order.strict_trans le_less_trans less.prems(3) prod.collapse state_wellFormed_init)
+
+            show "\<And>x. get_action (trace ! (i_switch - Suc 0)) = AInvoc x \<Longrightarrow> False"
+              using \<open>i_begin \<le> i_switch - Suc 0\<close> a2 allowed_context_switch_simps(6) le_eq_less_or_eq no_earlier_context_switches by fastforce
+          qed
+
+
+        have [simp]: "(Suc (i_switch - Suc 0)) = i_switch"
+          by (simp add: \<open>0 < i_switch\<close>)
+
+        show "(~~ initialState program \<leadsto>*) (take (i_switch - 1) trace @ drop (Suc (i_switch - 1)) trace) =
+              (~~ initialState program \<leadsto>*) (take (i_switch - 1) trace @ drop i_switch trace)"
+          by simp
+
+        show "i_switch - 1 < length trace"
+          by (simp add: a1 less_imp_diff_less)
+
+        show "state_wellFormed (initialState program)"
+          by (simp add: state_wellFormed_init)
+
+        show "\<And>i. (i, ACrash) \<notin> set trace"
+          by (simp add: less.prems(3))
+
+        text "As we are in the middle of a transaction, we cannot execute BeginAtomic or Invoc (packed)"
+        from `packed_trace trace`
+        show "\<And>j. \<lbrakk>i_switch - 1 < j; j < length trace\<rbrakk> \<Longrightarrow> get_invoc (trace ! j) \<noteq> get_invoc (trace ! (i_switch - 1))"
+          by (metis One_nat_def Suc_lessI \<open>0 < i_switch\<close> \<open>Suc (i_switch - Suc 0) = i_switch\<close> \<open>\<And>j'. \<lbrakk>i_switch < j'; j' < length trace\<rbrakk> \<Longrightarrow> get_invoc (trace ! j') \<noteq> invoc\<close> \<open>get_invoc (trace ! i_switch) \<noteq> invoc\<close> a0 diff_less less_Suc_eq_le same_invoc zero_less_one)
+
+      qed
+
+
+      show ?thesis
+      proof (rule less.hyps)
+        show "length trace' < length trace"
+          by (simp add: \<open>length trace = Suc (length trace')\<close>)
+        show "initialState program ~~ trace' \<leadsto>* S'"
+          by (simp add: \<open>initialState program ~~ trace' \<leadsto>* S'\<close>)
+        have [simp]: "min (length trace) i_switch = i_switch"
+          by (simp add: \<open>i_switch < length trace\<close> min_simps(2))
+        have [simp]: " i_switch + (length trace - Suc i_switch) = length trace - 1"
+          by (simp add: Suc_leI \<open>i_switch < length trace\<close>)
+        have [simp]: "min (length trace) (i_switch - Suc 0) = i_switch - Suc 0"
+          using \<open>i_switch < length trace\<close> by auto
+        have [simp]: "i_switch + (length trace - i_switch) = length trace"
+          by (simp add: \<open>i_switch < length trace\<close> less_imp_le)
+        have [simp]: "Suc (i_switch - Suc 0) = i_switch"
+          using Suc_pred \<open>0 < i_switch\<close> by blast
+
+
+        have h: "i = i_switch" if "i - Suc 0 < i_switch" and "\<not> i < i_switch" for i
+          using that(1) that(2) by linarith
+
+        show "packed_trace trace'"
+          using `packed_trace trace`
+          apply (auto simp add: packed_trace_def trace'_def  nth_append split: if_splits)
+          by (metis \<open>Suc (i_switch - Suc 0) = i_switch\<close> a4 h less_SucI linorder_neqE_nat not_less_eq)
+        show "\<And>s. (s, ACrash) \<notin> set trace'"
+          by (metis Un_iff append_take_drop_id less.prems(3) set_append trace'_def)
+
+
+        thm no_context_switch_transaction2
+
+        from `initialState program ~~ trace \<leadsto>* S`
+        have is_invoc: "get_invoc (trace ! (i_switch - 1)) = invoc"
+          using `trace ! i_begin = (invoc, ABeginAtomic tx txns)`
+        proof (rule no_context_switch_transaction2)
+          show "\<And>j. \<lbrakk>i_begin < j; j \<le> i_switch - 1\<rbrakk> \<Longrightarrow> trace ! j \<noteq> (invoc, AEndAtomic)"
+            by (simp add: a3)
+          show "packed_trace trace"
+            by (simp add: less.prems(2))
+          show "\<not> allowed_context_switch (get_action (trace ! j))" if "i_begin < j" "j \<le> i_switch - 1" for j
+          proof 
+            assume "allowed_context_switch (get_action (trace ! j))"
+            have "i_switch \<le> j"
+            proof (rule i_switch_min[where i_begin'=i_begin and i_switch'=j])
+              show "contextSwitchInTransaction trace i_begin j"
+              proof (auto simp add: contextSwitchInTransaction_def)
+                show "i_begin < j"
+                  by (simp add: that(1))
+                show "j < length trace"
+                  using a1 that(2) by auto
+                show "\<exists>invoc.
+                   (\<exists>tx txns. trace ! i_begin = (invoc, ABeginAtomic tx txns)) \<and>
+                   (\<forall>ja. i_begin < ja \<and> ja < j \<longrightarrow> trace ! ja \<noteq> (invoc, AEndAtomic)) \<and> allowed_context_switch (get_action (trace ! j))"
+                proof (intro exI conjI allI impI)
+                  show "trace ! i_begin = (invoc, ABeginAtomic tx txns)"
+                    by (simp add: a2)
+                  show "allowed_context_switch (get_action (trace ! j))"
+                    by (simp add: \<open>allowed_context_switch (get_action (trace ! j))\<close>)
+                  show "\<And>ja. i_begin < ja \<and> ja < j \<Longrightarrow> trace ! ja \<noteq> (invoc, AEndAtomic)"
+                    using a3 that(2) by auto
                 qed
               qed
             qed
-            then have "y < Suc pos"
-              using Suc_le_lessD m_max by blast
-            then have False
-              using \<open>pos < y\<close> not_less_eq by blast
-          }
-          then show "y < Suc pos"
-            using not_less_eq by blast
-        qed
-        show "\<exists>S_newEnd. initialState program ~~ newTrace \<leadsto>* S_newEnd"
-        proof -
-          
-          have "trace' = take pos trace' @ [trace'!pos] @ drop (Suc pos) trace'"
-            by (simp add: \<open>pos < length trace'\<close> id_take_nth_drop)
-
-          with \<open>initialState program ~~ trace' \<leadsto>* s\<close>
-          obtain S_pos S_pos2 S_end 
-            where S_pos_steps: "initialState program ~~ take pos trace' \<leadsto>* S_pos"
-              and S_pos_step: "S_pos ~~ trace'!pos \<leadsto> S_pos2"
-              and S_pos2_steps: "S_pos2 ~~ drop (Suc pos) trace' \<leadsto>* S_end"
-            by (smt append_Cons self_append_conv2 steps_append steps_appendFront)
-
-          then have S_pos2_steps_initial: "initialState program ~~ take (Suc pos) trace' \<leadsto>* S_pos2"
-            by (metis \<open>pos < length trace'\<close> steps_step take_Suc_conv_app_nth)
-
-
-
-          define invoc where "invoc = get_invoc(trace'!pos)"
-
-          from \<open>trace' ! j = (get_invoc (trace' ! pos), ABeginAtomic tx txns)\<close>
-          have beginAtomic: "trace' ! j = (invoc, ABeginAtomic tx txns)"
-            by (simp add: invoc_def)
-
-          from \<open>\<forall>k<length trace'. j < k \<longrightarrow> trace' ! k \<noteq> (get_invoc (trace' ! pos), AEndAtomic)\<close>
-          have noEndAtomic: "\<And>k. \<lbrakk>k<length trace'; j < k\<rbrakk> \<Longrightarrow> trace' ! k \<noteq> (invoc, AEndAtomic)"
-            by (simp add: invoc_def)
-
-          have inTx: "currentTransaction S_pos2 invoc \<noteq> None"
-          proof (rule inTransaction_trace[OF S_pos2_steps_initial])
-
-            from \<open>trace' ! j = (invoc, ABeginAtomic tx txns)\<close>
-            show "take (Suc pos) trace' ! j = (invoc, ABeginAtomic tx txns)"
-              by (simp add: \<open>j \<le> pos\<close> le_imp_less_Suc)
-
-            show "j < length (take (Suc pos) trace')"
-              by (simp add: Suc_leI \<open>j \<le> pos\<close> \<open>pos < length trace'\<close> le_imp_less_Suc min.absorb2)
-
-            show "\<And>k. \<lbrakk>k < length (take (Suc pos) trace'); j < k\<rbrakk> \<Longrightarrow> take (Suc pos) trace' ! k \<noteq> (invoc, AEndAtomic)"
-              by (simp add: noEndAtomic)
-
-            show "\<And>i. (i, ACrash) \<notin> set (take (Suc pos) trace')"
-              by (meson in_set_takeD less.prems(3))
+            thus False
+              using \<open>Suc (i_switch - Suc 0) = i_switch\<close> that(2) by auto
           qed
 
-          
-          
-
-          
-
-          obtain pos_action where pos_action_def[simp]: "trace'!pos = (invoc, pos_action)"
-            by (metis invoc_def prod.collapse)
-
-          from S_pos_step
-          have S_pos_step': "S_pos ~~ (invoc, pos_action) \<leadsto> S_pos2" 
-            by simp
-
-          have other_invocation: "\<And>a. a \<in> set (drop (Suc pos) trace') \<Longrightarrow> get_invoc a \<noteq> invoc"
-            using \<open>invoc = get_invoc (trace' ! pos)\<close> \<open>min (length trace') pos = pos\<close> \<open>\<And>pos'. \<lbrakk>pos < pos'; pos' < length trace'\<rbrakk> \<Longrightarrow> get_invoc (trace' ! pos') \<noteq> get_invoc (trace' ! pos)\<close>
-            by (auto simp add: in_set_conv_nth,
-             metis Suc_leI add_Suc fst_conv le_add_diff_inverse less_add_Suc1 nat_add_left_cancel_less pos_less)
-
-          have other_invocation'[simp]: "\<And>a. (invoc, a) \<notin> set (drop (Suc pos) trace')" 
-            by (meson fst_conv other_invocation)
-
-
-          from \<open>S_pos2 ~~ drop (Suc pos) trace' \<leadsto>* S_end\<close>
-          have S_pos_steps_to_S_end: "S_pos ~~ (invoc, pos_action) # drop (Suc pos) trace' \<leadsto>* S_end"
-            using S_pos_step' steps_appendFront by blast
-
-
-          from \<open>initialState program ~~ take pos trace' \<leadsto>* S_pos\<close>
-          have S_pos_wf[simp]: "state_wellFormed S_pos"
-            using state_wellFormed_combine state_wellFormed_init
-            by (metis contra_subsetD less.prems(3) set_take_subset) 
-
-          have "\<exists>S_new_end. S_pos ~~ drop (Suc pos) trace' \<leadsto>* S_new_end"
-          proof (cases "pos_action")
-            case ALocal
-            then have [simp]: "pos_action = ALocal" by simp
-
-            show ?thesis
-              by (rule exI, 
-                  rule remove_local_step[OF S_pos_step' S_pos_steps_to_S_end S_pos2_steps],
-                  auto simp add: other_invocation)
-
-          next
-            case (ANewId x2)
-
-            show ?thesis 
-              by (rule exI,
-                  rule remove_newId_step[OF S_pos_steps_to_S_end S_pos_step' S_pos2_steps],
-                  auto simp add: other_invocation ANewId)
-
-          next
-            case (ABeginAtomic x31 x32)
-
-            
-
-            show ?thesis
-              by (rule exI,
-              rule remove_beginAtomic_step[OF S_pos_steps_to_S_end S_pos_step' S_pos2_steps],
-              auto simp add: other_invocation ABeginAtomic)
-
-          next
-            case AEndAtomic
-            then show ?thesis 
-              using \<open>j \<le> pos\<close> \<open>pos < length trace'\<close> local.beginAtomic noEndAtomic by fastforce
-          next
-            case (ADbOp )
-            show ?thesis 
-              by (rule exI,
-                  rule remove_DBOp_step[OF S_pos_steps_to_S_end S_pos_step' S_pos2_steps],
-                  auto simp add: other_invocation ADbOp)
-          next
-            case (AInvoc)
-
-            \<comment> \<open>We already have an beginAtomic before, so we already have an invocId\<close>
-            have "invocationOp S_pos invoc \<noteq> None"
-            proof -
-
-              have f4: "j < length (take pos trace')"
-                using AInvoc Pair_inject j_leq_pos le_eq_less_or_eq local.beginAtomic by auto
-              have f5: "take pos trace' ! j = (get_invoc (trace' ! pos), ABeginAtomic tx txns)"
-                using AInvoc Pair_inject j_leq_pos le_eq_less_or_eq local.beginAtomic by auto
-
-              have "currentTransaction S_pos (get_invoc (trace' ! pos)) \<noteq> None"
-                using [[smt_timeout=60]]
-                by (smt S_pos_steps \<open>min (length trace') pos = pos\<close> f4 f5 inTransaction_trace in_set_takeD length_take less.prems(3) less_trans noEndAtomic_trace' nth_take pos_less)
-              then show ?thesis
-                by (metis S_pos_wf invoc_def wellFormed_invoc_notStarted(1))
-            qed
-
-
-
-            with AInvoc
-            show ?thesis
-              using S_pos_step inTx by (auto simp add: step.simps inTx)
-          next
-            case (AReturn x7)
-            then show ?thesis 
-              using S_pos_step inTx by (auto simp add: step.simps inTx)
-          next
-            case ACrash
-            then show ?thesis
-              using \<open>pos < length trace'\<close> \<open>\<And>s. (s, ACrash) \<notin> set trace'\<close> nth_mem by fastforce
-          next
-            case (AInvcheck x92)
-            then have "S_pos2 = S_pos"
-              using S_pos_step by (auto simp add: step.simps)
-            with \<open>S_pos2 ~~ drop (Suc pos) trace' \<leadsto>* S_end\<close> 
-            show ?thesis by blast
-          qed
-
-
-          with \<open>initialState program ~~ take pos trace' \<leadsto>* S_pos\<close>
-          show "\<exists>S_newEnd. initialState program ~~ newTrace \<leadsto>* S_newEnd"
-            by (auto simp add: newTrace_def  steps_append)
+          show "i_begin \<le> i_switch - 1"
+            using a0 by auto
+          show "i_switch - 1 < length trace"
+            using a1 less_imp_diff_less by blast
         qed
 
-        show "packed_trace newTrace"
-          using \<open>packed_trace trace'\<close> 
-        proof (auto simp add: newTrace_def packed_trace_def nth_append)
-
-
-          show "allowed_context_switch (get_action (trace' ! i))"
-            if c0: "\<forall>i>0. i < length trace' \<longrightarrow> get_invoc (trace' ! (i - Suc 0)) \<noteq> get_invoc (trace' ! i) \<longrightarrow> allowed_context_switch (get_action (trace' ! i))"
-              and c1: "i - Suc 0 < pos"
-              and c2: "i < pos"
-              and c3: "0 < i"
-              and c4: "get_invoc (trace' ! (i - Suc 0)) \<noteq> get_invoc (trace' ! i)"
-            for  i
-            using \<open>pos < length trace'\<close> dual_order.strict_trans that by blast
-
-
-          show "allowed_context_switch (get_action (trace' ! Suc i))"
-            if c0: "\<forall>i>0. i < length trace' \<longrightarrow> get_invoc (trace' ! (i - Suc 0)) \<noteq> get_invoc (trace' ! i) \<longrightarrow> allowed_context_switch (get_action (trace' ! i))"
-              and c1: "i - Suc 0 < pos"
-              and c2: "\<not> i < pos"
-              and c3: "i < pos + (length trace' - Suc pos)"
-              and c4: "get_invoc (trace' ! (i - Suc 0)) \<noteq> get_invoc (trace' ! Suc i)"
-            for  i
-            using that by (metis (no_types, hide_lams) Suc_pred diff_Suc_Suc diff_zero less_add_same_cancel1 maxPos not_gr_zero not_less_eq not_less_less_Suc_eq zero_less_Suc zero_less_diff)
-        qed
-        show " \<And>s. (s, ACrash) \<notin> set newTrace"
-          using \<open>\<And>s. (s, ACrash) \<notin> set trace'\<close> by (auto simp add: newTrace_def dest: in_set_takeD in_set_dropD )
-
-        show "no_invariant_checks_in_transaction newTrace"
-        proof (cases "get_action (trace' ! pos) \<noteq> AEndAtomic")
-          case True
-          show ?thesis 
-            unfolding newTrace_def
-            by (rule maintain_no_invariant_checks_in_transaction[OF \<open>no_invariant_checks_in_transaction trace'\<close> True \<open>pos < length trace'\<close>])
-          next
-            case False
-            with \<open>no_invariant_checks_in_transaction trace'\<close>
-            show ?thesis 
-              by (cases "trace' ! pos",
-                  insert beginAtomic_trace' j_leq_pos le_eq_less_or_eq noEndAtomic_trace' pos_less,
-                  auto simp add: newTrace_def no_invariant_checks_in_transaction_def nth_append)
-          qed
+        from `no_invariant_checks_in_transaction trace`
+        have "no_invariant_checks_in_transaction (take (i_switch - 1) trace @ drop (Suc (i_switch - 1)) trace)"
+        proof (rule maintain_no_invariant_checks_in_transaction2)
+          show "i_switch - 1 < length trace"
+            by (simp add: \<open>i_switch < length trace\<close> less_imp_diff_less)
+          show "
+           \<lbrakk>i < i_switch - 1; trace ! i = (invoc, ABeginAtomic tx txns); \<And>ja. \<lbrakk>i < ja; ja < i_switch - 1\<rbrakk> \<Longrightarrow> trace ! ja \<noteq> (invoc, AEndAtomic)\<rbrakk>
+             \<Longrightarrow> trace ! (i_switch - 1) \<noteq> (invoc, AEndAtomic)" for i invoc tx txns
+              by (metis One_nat_def \<open>Suc (i_switch - Suc 0) = i_switch\<close> is_invoc a0 a2 a3 action.distinct(31) fst_conv le_eq_less_or_eq less_Suc_eq_le snd_conv)
         qed
 
-\<comment> \<open>because no inv-checks in transaction\<close>
-      have removedNoInvCheck: "get_action (trace'!pos) \<noteq> AInvcheck v" for v
-        
-        using \<open>no_invariant_checks_in_transaction trace'\<close>
-        by (auto simp add: no_invariant_checks_in_transaction_def,
-            smt \<open>pos < length trace' \<and> (\<exists>i j tx txns. get_invoc (trace' ! pos) = i \<and> j \<le> pos \<and> trace' ! j = (i, ABeginAtomic tx txns) \<and> \<not> (\<exists>k>j. k < length trace' \<and> trace' ! k = (i, AEndAtomic)))\<close> allowed_context_switch_def allowed_context_switch_simps(9) le_eq_less_or_eq min_def min_less_iff_conj prod.collapse prod.inject)
-
-
-
-      show "traceCorrect trace'"
-      proof (auto simp add: traceCorrect_def newTrace_def in_set_conv_nth)
-        fix s i
-        assume  "i < length trace'" and "trace' ! i = (s, AInvcheck False)"
-
-        {
-          assume "i<pos"
-          then have "newTrace ! i \<noteq> (s, AInvcheck False)"
-            using \<open>traceCorrect newTrace\<close> \<open>pos < length trace'\<close> newTrace_def \<open>trace' ! i = (s, AInvcheck False)\<close> by (auto simp add: traceCorrect_def in_set_conv_nth)
-          then have "trace' ! i \<noteq> (s, AInvcheck False)"
-            using \<open>i < pos\<close> \<open>pos < length trace'\<close> newTraceIth newTraceLen by force
-        }
-        moreover
-        {
-          assume "i = pos"
-          then have "newTrace ! i \<noteq> (s, AInvcheck False)"
-            using \<open>trace' ! i = (s, AInvcheck False)\<close> removedNoInvCheck by auto
-          then have "trace' ! i \<noteq> (s, AInvcheck False)"
-            using \<open>i = pos\<close> removedNoInvCheck by fastforce
-        }
-        moreover
-        {
-          assume "i>pos"
-          then have "newTrace ! i \<noteq> (s, AInvcheck False)"
-            by (smt Suc_leI Suc_less_SucD \<open>i < length trace'\<close> \<open>trace' ! i = (s, AInvcheck False)\<close> \<open>traceCorrect newTrace\<close> diff_Suc_1 in_set_conv_nth leD less_imp_Suc_add newTraceIth newTraceLen traceCorrect_def)
-          then have "trace' ! i \<noteq> (s, AInvcheck False)"
-            by (smt Suc_leI Suc_less_SucD \<open>i < length trace'\<close> \<open>pos < i\<close> \<open>traceCorrect newTrace\<close> diff_Suc_1 in_set_conv_nth leD less_imp_Suc_add newTraceIth newTraceLen traceCorrect_def)
-        }
-        ultimately have "trace' ! i \<noteq> (s, AInvcheck False)"
-          using antisym_conv3 by blast
-        then show False
-          using \<open>trace' ! i = (s, AInvcheck False)\<close> by blast
+        show " no_invariant_checks_in_transaction trace'"
+          using maintain_no_invariant_checks_in_transaction[OF `no_invariant_checks_in_transaction trace`, where pos="i_switch - 1", simplified]
+          using One_nat_def \<open>Suc (i_switch - Suc 0) = i_switch\<close> \<open>no_invariant_checks_in_transaction (take (i_switch - 1) trace @ drop (Suc (i_switch - 1)) trace)\<close> trace'_def by presburger
+        show "\<not> traceCorrect trace'"
+          using `\<not>traceCorrect trace` trace'_def
+          apply (auto simp add: traceCorrect_def)
+          by (metis (no_types, lifting) Suc_diff_Suc UnI2 \<open>i_switch + (length trace - Suc i_switch) = length trace - 1\<close> \<open>i_switch + (length trace - i_switch) = length trace\<close> \<open>length trace = Suc (length trace')\<close> \<open>length trace' < length trace\<close> a1 add_less_cancel_left diff_Suc_1 diff_is_0_eq last_action_incorrect last_conv_nth last_drop leD length_drop list.size(3) nth_mem)
+        show "initialState program ~~ trace' \<leadsto>* S'"
+          by (simp add: \<open>initialState program ~~ trace' \<leadsto>* S'\<close>)
+        show "packed_trace trace'"
+          by (simp add: \<open>packed_trace trace'\<close>)
+        show "\<And>s. (s, ACrash) \<notin> set trace'"
+          by (simp add: \<open>\<And>s. (s, ACrash) \<notin> set trace'\<close>)
+        show "no_invariant_checks_in_transaction trace'"
+          by (simp add: \<open>no_invariant_checks_in_transaction trace'\<close>)
+        show " \<not> traceCorrect trace'"
+          by (simp add: \<open>\<not> traceCorrect trace'\<close>)
+        show "\<And>s. (s, AInvcheck True) \<notin> set trace'"
+          by (metis Un_iff append_take_drop_id less.prems(4) set_append trace'_def)
+        thus "\<And>s. (s, AInvcheck True) \<notin> set trace'" .
       qed
     qed
   qed
 qed
 
+theorem show_programCorrect_noTransactionInterleaving'':
+  assumes packedTracesCorrect: 
+    "\<And>trace s. \<lbrakk>
+      initialState program ~~ trace \<leadsto>* s; 
+      packed_trace trace; 
+      \<not>contextSwitchesInTransaction trace;  
+      \<And>s. (s, ACrash) \<notin> set trace; 
+      no_invariant_checks_in_transaction trace
+    \<rbrakk> \<Longrightarrow> traceCorrect trace"
+  shows "programCorrect program"
+proof (rule show_programCorrect_noTransactionInterleaving', rule ccontr, goal_cases g)
+  case (g trace s)
+  obtain trace s
+    where "initialState program ~~ trace \<leadsto>* s"
+      "packed_trace trace"
+      "\<not>contextSwitchesInTransaction trace"
+      "\<And>s. (s, ACrash) \<notin> set trace"
+      "no_invariant_checks_in_transaction trace"
+      "\<not>traceCorrect trace"
+    using remove_context_switches_in_transactions[OF g]
+    by metis
+
+
+  then show ?case
+    using packedTracesCorrect by blast 
+qed
 
 
 
