prefix.thy
@@ -20,6 +20,9 @@ lemma isPrefix_refl: "isPrefix xs xs"
 lemma isPrefix_empty: "isPrefix xs [] \<longleftrightarrow> xs = []"
   by (simp add: isPrefix_def)
 
+lemma isPrefix_empty_first: "isPrefix [] xs"
+  by (simp add: isPrefix_def)
+
 lemma isPrefix_appendI:
   "isPrefix xs (xs@ys)"
   by (simp add: isPrefix_def)
@@ -27,6 +30,25 @@ lemma isPrefix_appendI:
 lemma isPrefix_len:
   "isPrefix tr tr' \<Longrightarrow> length tr \<le> length tr'"
   by (metis isPrefix_def nat_le_linear take_all)
+
+lemma isPrefix_trans:
+  "isPrefix xs ys \<Longrightarrow> isPrefix ys zs \<Longrightarrow> isPrefix xs zs"
+  by (auto simp add: isPrefix_def, metis length_take take_take)
+
+
+lemma isPrefix_appendPrefix:
+  "isPrefix (xs@ys) zs \<Longrightarrow> isPrefix xs zs"
+  using isPrefix_appendI isPrefix_trans by blast
+
+lemma isPrefix_subset:
+  "isPrefix xs ys \<Longrightarrow> set xs \<subseteq> set ys"
+  by (metis isPrefix_def set_take_subset)
+
+lemma isPrefix_subset2:
+  "isPrefix xs ys \<Longrightarrow> x\<in>set xs \<Longrightarrow> x\<in> set ys"
+  using isPrefix_subset by auto
+
+
 
 
 lemma isPrefix_same: 
